common/theories/LoopChecking/HornClauses.v
@@ -5,7 +5,7 @@ From Stdlib Require Import Orders OrderedTypeAlt OrderedTypeEx MSetList MSetInte
 From MetaRocq.Utils Require Import utils.
 
 From MetaRocq.Common Require Universes.
-From MetaRocq.Common Require Import Interfaces.
+From MetaRocq.Common Require Import Common Interfaces.
 From Equations Require Import Equations.
 Set Equations Transparent.
 
@@ -84,12 +84,15 @@ Module Clauses (LS : LevelSets).
   Module ClausesFact := WFactsOn Clause Clauses.
   Module ClausesProp := WPropertiesOn Clause Clauses.
   Module ClausesDecide := WDecide (Clauses).
+  Module ClausesOrd := OrdProperties Clauses.
+
   Ltac clsets := ClausesDecide.fsetdec.
   Infix "⊂_clset" := Clauses.Subset (at level 70).
+  Infix "=_clset" := Clauses.Equal (at level 70).
 
   Definition clauses := Clauses.t.
 
-  Lemma filter_add {p x s} : Clauses.Equal (Clauses.filter p (Clauses.add x s)) (if p x then Clauses.add x (Clauses.filter p s) else Clauses.filter p s).
+  Lemma filter_add {p x s} : Clauses.filter p (Clauses.add x s) =_clset if p x then Clauses.add x (Clauses.filter p s) else Clauses.filter p s.
   Proof.
     intros i.
     rewrite Clauses.filter_spec.
@@ -125,31 +128,6 @@ Module Clauses (LS : LevelSets).
       destruct (p x) eqn:px => //.
       rewrite ClausesProp.fold_add //.
       rewrite Clauses.filter_spec. intuition auto.
-  Qed.
-
-  Definition strict_subset (s s' : LevelSet.t) :=
-    LevelSet.Subset s s' /\ ~ LevelSet.Equal s s'.
-
-  Lemma strict_subset_incl (x y z : LevelSet.t) : LevelSet.Subset x y -> strict_subset y z -> strict_subset x z.
-  Proof.
-    intros hs []. split => //. lsets.
-    intros heq. apply H0. lsets.
-  Qed.
-
-  Lemma strict_subset_cardinal s s' : strict_subset s s' -> LevelSet.cardinal s < LevelSet.cardinal s'.
-  Proof.
-    intros [].
-    assert (LevelSet.cardinal s <> LevelSet.cardinal s').
-    { intros heq. apply H0.
-      intros x. split; intros. now apply H.
-      destruct (LevelSet.mem x s) eqn:hin.
-      eapply LevelSet.mem_spec in hin.
-      auto. eapply LevelSetProp.FM.not_mem_iff in hin.
-      exfalso.
-      eapply LevelSetProp.subset_cardinal_lt in hin; tea.
-      lia. }
-    enough (LevelSet.cardinal s <= LevelSet.cardinal s') by lia.
-    now eapply LevelSetProp.subset_cardinal.
   Qed.
 
   Definition premise (cl : clause) := fst cl.
@@ -490,5 +468,897 @@ Module Clauses (LS : LevelSets).
     intuition eauto. destruct H as [cl []]; exists cl; split; try clsets; auto.
   Qed.
 
+  Lemma clauses_levels_conclusions cls V : clauses_levels cls ⊂_lset V ->
+    clauses_conclusions cls ⊂_lset V.
+  Proof.
+    intros hin x; rewrite clauses_conclusions_spec; move => [cl [hin' eq]]; apply hin.
+    rewrite clauses_levels_spec. exists cl. split => //. subst x.
+    rewrite clause_levels_spec. now right.
+  Qed.
+
+  Definition clauses_premises_levels (cls : clauses) : LevelSet.t :=
+    Clauses.fold (fun cl acc => LevelSet.union (levels (premise cl)) acc) cls LevelSet.empty.
+
+  Lemma clauses_premises_levels_spec_aux l cls acc :
+    LevelSet.In l (Clauses.fold (fun cl acc => LevelSet.union (levels (premise cl)) acc) cls acc) <->
+    (exists cl, Clauses.In cl cls /\ LevelSet.In l (levels (premise cl))) \/ LevelSet.In l acc.
+  Proof.
+    eapply ClausesProp.fold_rec.
+    - intros.
+      intuition auto. destruct H1 as [k [hin hl]]. clsets.
+    - intros x a s' s'' hin nin hadd ih.
+      rewrite LevelSet.union_spec.
+      split.
+      * intros [hin'|].
+        left. exists x. split => //.
+        apply hadd. now left.
+        apply ih in H.
+        intuition auto.
+        left. destruct H0 as [k Hk]. exists k. intuition auto. apply hadd. now right.
+      * intros [[k [ins'' ?]]|inacc].
+        eapply hadd in ins''. destruct ins''; subst.
+        + now left.
+        + right. apply ih. now left; exists k.
+        + right. intuition auto.
+  Qed.
+
+  Lemma clauses_premises_levels_spec l cls :
+    LevelSet.In l (clauses_premises_levels cls) <->
+    exists cl, Clauses.In cl cls /\ LevelSet.In l (levels (premise cl)).
+  Proof.
+    unfold clauses_premises_levels.
+    rewrite clauses_premises_levels_spec_aux.
+    intuition auto. lsets.
+  Qed.
+
+  Lemma clauses_levels_premises cls V : clauses_levels cls ⊂_lset V ->
+    clauses_premises_levels cls ⊂_lset V.
+  Proof.
+    intros hin x; rewrite clauses_premises_levels_spec; move => [cl [hin' eq]]; apply hin.
+    rewrite clauses_levels_spec. exists cl. split => //.
+    rewrite clause_levels_spec. now left.
+  Qed.
+
+  Lemma clauses_premises_levels_incl cls : clauses_premises_levels cls ⊂_lset clauses_levels cls.
+  Proof.
+    intros x; rewrite clauses_premises_levels_spec clauses_levels_spec; move => [cl [hin' eq]].
+    exists cl; split => //.
+    rewrite clause_levels_spec. now left.
+  Qed.
+
+  Lemma clauses_premises_levels_mon {cls cls'} : cls ⊂_clset cls' ->
+    clauses_premises_levels cls ⊂_lset clauses_premises_levels cls'.
+  Proof.
+    intros hin x; rewrite !clauses_premises_levels_spec; move => [cl [hin' eq]].
+    exists cl; split => //. now apply hin.
+  Qed.
+
+  Definition monotone_selector sel :=
+    forall cls' cls, cls' ⊂_clset cls -> sel cls' ⊂_lset sel cls.
+
+  Lemma clauses_levels_mon : monotone_selector clauses_levels.
+  Proof.
+    intros cls' cls hin x; rewrite !clauses_levels_spec; move => [cl [hin' eq]].
+    exists cl; split => //. now apply hin.
+  Qed.
+
+  Lemma clauses_with_concl_union cls W W' :
+    Clauses.Equal (cls ↓ (W ∪ W'))
+      (Clauses.union (cls ↓ W) (cls ↓ W')).
+  Proof.
+    intros x. rewrite Clauses.union_spec !in_clauses_with_concl LevelSet.union_spec.
+    firstorder.
+  Qed.
+
+  Lemma clauses_with_concl_subset cls W : (cls ↓ W) ⊂_clset cls.
+  Proof. now intros ?; rewrite in_clauses_with_concl. Qed.
+
+  Lemma union_diff_eq {cls cls'} : Clauses.Equal (Clauses.union cls (Clauses.diff cls' cls))
+    (Clauses.union cls cls').
+  Proof. clsets. Qed.
+
+  Lemma union_restrict_with_concl {cls W} :
+    Clauses.Equal (Clauses.union (cls ⇂ W) (cls ↓ W)) (cls ↓ W).
+  Proof.
+    intros cl. rewrite Clauses.union_spec.
+    intuition auto.
+    eapply in_clauses_with_concl.
+    now eapply in_restrict_clauses in H0 as [].
+  Qed.
+
+  Lemma union_diff {cls W} :
+    Clauses.Equal (Clauses.union (Clauses.diff (cls ↓ W) (cls ⇂ W)) (cls ⇂ W)) (cls ↓ W).
+  Proof.
+    now rewrite ClausesProp.union_sym union_diff_eq union_restrict_with_concl.
+  Qed.
+
+  Lemma union_diff_cls {cls W} :
+    Clauses.Equal (Clauses.union (Clauses.diff (cls ↓ W) (cls ⇂ W)) cls) cls.
+  Proof.
+    intros ?. rewrite Clauses.union_spec Clauses.diff_spec in_restrict_clauses in_clauses_with_concl.
+    firstorder.
+  Qed.
+
+  Lemma clauses_partition_spec {cls W allW conclW} :
+    clauses_conclusions cls ⊂_lset W ->
+    Clauses.partition (premise_restricted_to W) cls = (allW, conclW) ->
+    (Clauses.Equal allW (cls ⇂ W)) /\
+    (Clauses.Equal conclW (Clauses.diff cls (cls ⇂ W))).
+  Proof.
+    intros clW.
+    destruct Clauses.partition eqn:eqp.
+    intros [= <- <-].
+    change t with (t, t0).1.
+    change t0 with (t, t0).2 at 2.
+    rewrite -eqp. clear t t0 eqp.
+    split.
+    - intros cl. rewrite Clauses.partition_spec1.
+      rewrite in_restrict_clauses Clauses.filter_spec.
+      rewrite /premise_restricted_to LevelSet.subset_spec. firstorder eauto.
+      apply clW, clauses_conclusions_spec. now exists cl.
+    - intros cl. rewrite Clauses.partition_spec2.
+      rewrite Clauses.filter_spec Clauses.diff_spec.
+      rewrite /premise_restricted_to. intuition auto.
+      move/negbTE: H1. eapply eq_true_false_abs.
+      eapply LevelSet.subset_spec.
+      now eapply in_restrict_clauses in H as [].
+      apply eq_true_not_negb. move/LevelSet.subset_spec => he.
+      apply H1. apply in_restrict_clauses. split => //.
+      apply clW, clauses_conclusions_spec. now exists cl.
+  Qed.
+
+  Lemma clauses_conclusions_eq cls W :
+    clauses_conclusions cls ⊂_lset W ->
+    Clauses.Equal cls (cls ↓ W).
+  Proof.
+    intros cl x.
+    rewrite in_clauses_with_concl. intuition auto.
+    apply cl, clauses_conclusions_spec. now exists x.
+  Qed.
+
+  Definition levelexprset_of_levels (ls : LevelSet.t) n : LevelExprSet.t :=
+    LevelSet.fold (fun x => LevelExprSet.add (x, n)) ls LevelExprSet.empty.
+
+  Lemma levelexprset_of_levels_spec {ls : LevelSet.t} {l k n} :
+    LevelExprSet.In (l, k) (levelexprset_of_levels ls n) <-> LevelSet.In l ls /\ k = n.
+  Proof.
+    rewrite /levelexprset_of_levels.
+    eapply LevelSetProp.fold_rec.
+    - intros s' he. rewrite LevelExprSetFact.empty_iff. firstorder.
+    - intros x a s' s'' hin hnin hadd ih.
+      rewrite LevelExprSet.add_spec; unfold LevelExprSet.E.eq.
+      firstorder eauto; try noconf H1 => //.
+      apply hadd in H1. firstorder. subst. now left.
+  Qed.
+
+  #[program]
+  Definition of_level_set (ls : LevelSet.t) n (hne : ~ LevelSet.Empty ls) : premises :=
+    {| t_set := levelexprset_of_levels ls n |}.
+  Next Obligation.
+    apply not_Empty_is_empty => he. apply hne.
+    intros l nin. specialize (he (l,n)). apply he.
+    now rewrite levelexprset_of_levels_spec.
+  Qed.
+
+  Lemma of_level_set_union_spec {ls ls' n hne} hne' hne'' :
+    of_level_set (ls ∪ ls') n hne =
+    univ_union (of_level_set ls n hne') (of_level_set ls' n hne'').
+  Proof.
+    apply eq_univ_equal.
+    intros [l k]. rewrite /of_level_set //= !levelexprset_of_levels_spec LevelExprSet.union_spec.
+    rewrite !levelexprset_of_levels_spec LevelSet.union_spec. clear. firstorder.
+  Qed.
+
+  Lemma of_level_set_singleton l k hne : of_level_set (LevelSet.singleton l) k hne = singleton (l, k).
+  Proof.
+    apply eq_univ_equal. move=> [l' k'].
+    rewrite /of_level_set //= levelexprset_of_levels_spec !LevelExprSet.singleton_spec LevelSet.singleton_spec /LevelSet.E.eq /LevelExprSet.E.eq.
+    firstorder subst => //. now noconf H. now noconf H.
+  Qed.
+
+  Definition max_premise_of l (u : premises) : option Z :=
+    LevelExprSet.fold (fun '(l', k) acc => if eqb l l' then
+      max_opt_of Z.max (Some k) acc else acc) u None.
+
+  Lemma max_premise_of_spec l k (u : premises) : LevelExprSet.In (l, k) u -> Some k ≤ max_premise_of l u.
+  Proof.
+    rewrite /max_premise_of.
+    eapply LevelExprSetProp.fold_rec.
+    - intros s' he hin. now apply he in hin.
+    - intros x a s' s'' hin nin hadd hle.
+      intros hs''. destruct x.
+      apply hadd in hs'' as [].
+      * noconf H. rewrite eqb_refl. destruct a; cbn. constructor. lia. reflexivity.
+      * elim: eqb_spec; try intros ->;
+        specialize (hle H); depelim hle; cbn; constructor; lia.
+  Qed.
+
+  Definition max_clause_premise_of l (cls : clauses) :=
+    Clauses.fold (fun cl acc => max_opt_of Z.max (max_premise_of l (premise cl)) acc) cls None.
+
+  Lemma max_clause_premise_of_spec l k cls :
+    forall cl, Clauses.In cl cls -> LevelExprSet.In (l, k) (premise cl) -> Some k ≤ max_clause_premise_of l cls.
+  Proof.
+    rewrite /max_clause_premise_of => cl.
+    eapply ClausesProp.fold_rec.
+    - intros s' he hin. now apply he in hin.
+    - intros x a s' s'' hin nin hadd hle.
+      intros hs''. destruct x.
+      apply hadd in hs'' as [].
+      * noconf H. cbn. move/max_premise_of_spec.
+        intros h; etransitivity; tea. destruct (max_premise_of l n), a; cbn; constructor; lia.
+      * intros h; specialize (hle H h). depelim hle. cbn.
+        destruct (max_premise_of l n); cbn; constructor; lia.
+  Qed.
+
+  Definition max_clause_premises cls :=
+    let ls := clauses_levels cls in
+    let fn l m := LevelMap.add l (max_clause_premise_of l cls) m in
+    LevelSet.fold fn ls (LevelMap.empty _).
+
+  Lemma max_clause_premises_spec l k cls :
+    LevelMap.MapsTo l k (max_clause_premises cls) ->
+    LevelSet.In l (clauses_levels cls) /\ k = max_clause_premise_of l cls.
+  Proof.
+    unfold max_clause_premises.
+    eapply LevelSetProp.fold_rec.
+    - intros s' he hm. now rewrite LevelMapFact.F.empty_mapsto_iff in hm.
+    - intros x a s' s'' hin hnin hadd ih.
+      rewrite LevelMapFact.F.add_mapsto_iff.
+      intros [[-> [= <-]]|[]] => //.
+      * split => //. apply hadd. now left.
+      * split => //. apply hadd; now right. now apply ih.
+  Qed.
+
+  Lemma max_clause_premises_spec_inv cls :
+    forall l, LevelSet.In l (clauses_levels cls) ->
+    LevelMap.MapsTo l (max_clause_premise_of l cls) (max_clause_premises cls).
+  Proof.
+    unfold max_clause_premises.
+    eapply LevelSetProp.fold_rec.
+    - intros s' he hm. now move/he.
+    - intros x a s' s'' hin hnin hadd ih l ls''.
+      rewrite LevelMapFact.F.add_mapsto_iff.
+      destruct (eq_dec x l). subst.
+      * now left.
+      * right. split => //. apply ih. eapply hadd in ls''. destruct ls''; auto. contradiction.
+  Qed.
+
+  Local Open Scope Z_scope.
+
+  Definition add_expr n '((l, k) : LevelExpr.t) := (l, k + n).
+
+  Lemma add_expr_add_expr n n' lk : add_expr n (add_expr n' lk) = add_expr (n + n') lk.
+  Proof. destruct lk; unfold add_expr. f_equal; lia. Qed.
+  Definition add_prems n s := map (add_expr n) s.
+
+  Lemma In_add_prems k (prems : premises):
+    forall le, LevelExprSet.In le (add_prems k prems) <->
+      exists le', LevelExprSet.In le' prems /\ le = add_expr k le'.
+  Proof.
+    intros [l k'].
+    now rewrite /add_prems map_spec.
+  Qed.
+
+  Lemma add_expr_inj {n e e'} : add_expr n e = add_expr n e' -> e = e'.
+  Proof.
+    destruct e, e'; cbn; intros [=].
+    have eq: z = z0 by lia.
+    now subst z0.
+  Qed.
+
+  Lemma add_prems_inj n prems prems' : add_prems n prems = add_prems n prems' -> prems = prems'.
+  Proof.
+    rewrite /add_prems => /eq_univ_equal hm.
+    apply eq_univ_equal.
+    intros [l k]. specialize (hm (l, k + n)).
+    rewrite !map_spec in hm. destruct hm as [hl hr].
+    split; intros hin.
+    - forward hl. exists (l, k); split => //.
+      destruct hl as [[] [hin' eq]].
+      apply (@add_expr_inj n (l, k)) in eq. now noconf eq.
+    - forward hr. exists (l, k); split => //.
+      destruct hr as [[] [hin' eq]].
+      apply (@add_expr_inj n (l, k)) in eq. now noconf eq.
+  Qed.
+
+  Lemma add_prems_add_prems n n' lk : add_prems n (add_prems n' lk) = add_prems (n + n') lk.
+  Proof. destruct lk; unfold add_prems.
+    rewrite map_map. apply eq_univ_equal.
+    intros x. rewrite !map_spec. cbn in *.
+    firstorder eauto. subst. exists x0.
+    firstorder eauto. now rewrite add_expr_add_expr.
+    subst. exists x0.
+    firstorder eauto. now rewrite add_expr_add_expr.
+  Qed.
+
+  Lemma add_prems_add {n lk prems} : add_prems n (add lk prems) = add (add_expr n lk) (add_prems n prems).
+  Proof.
+    apply eq_univ_equal. intros x.
+    rewrite In_add_prems LevelExprSet.add_spec In_add_prems /LevelExprSet.E.eq; rw LevelExprSet.add_spec.
+    firstorder. subst. red in H; subst x0. now left.
+  Qed.
+
+  Lemma add_prems_0 u : add_prems 0 u = u.
+  Proof.
+    rewrite /add_prems.
+    apply eq_univ_equal.
+    intros x. rewrite map_spec.
+    split.
+    - intros[e [hin ->]]. unfold add_expr. now destruct e; rewrite Z.add_0_r.
+    - intros inu; exists x. split => //. destruct x. now rewrite /add_expr Z.add_0_r.
+  Qed.
+
+  Lemma add_prems_of_level_set k W k' prf :
+    add_prems k (of_level_set W k' prf) = of_level_set W (k + k') prf.
+  Proof.
+    apply eq_univ_equal => [] [l n].
+    rewrite In_add_prems /of_level_set //= levelexprset_of_levels_spec.
+    split.
+    - move=> [] [l' n']. rewrite levelexprset_of_levels_spec => [] [[inw eq] eq'].
+      subst n'. noconf eq'. split => //. lia.
+    - move=> [inW ->]. exists (l, k'). rewrite levelexprset_of_levels_spec.
+      split => //. cbn. f_equal; lia.
+  Qed.
+
+  Definition add_clause n '((prems, concl) : clause) := (add_prems n prems, add_expr n concl).
+
+  Lemma add_clause_add_clause n n' cl : add_clause n (add_clause n' cl) = add_clause (n + n') cl.
+  Proof.
+    destruct cl.
+    unfold add_clause.
+    now rewrite add_prems_add_prems add_expr_add_expr.
+  Qed.
+
+  Notation succ_expr := (add_expr 1).
+  Notation succ_prems := (add_prems 1).
+  Notation succ_clause := (add_clause 1).
+
+  Arguments add_prems : simpl never.
+
+  Lemma add_clause_inj {n x y} : add_clause n x = add_clause n y -> x = y.
+  Proof.
+    destruct x as [prems concl], y as [prems' concl']. cbn.
+    apply: pair_inj. now move=> /add_prems_inj -> /add_expr_inj ->.
+  Qed.
+  Definition add_clauses n cls := ClausesProp.of_list (List.map (fun cl => add_clause n cl) (ClausesProp.to_list cls)).
+  Notation succ_clauses := (add_clauses 1).
+  Import SetoidList.
+
+  Lemma add_clauses_spec {cl cls} n : Clauses.In cl cls <-> Clauses.In (add_clause n cl) (add_clauses n cls).
+  Proof.
+    unfold succ_clauses.
+    rewrite ClausesProp.of_list_1 InA_In_eq in_map_iff.
+    firstorder eauto.
+    - exists cl; split => //. unfold ClausesProp.to_list. now eapply Clauses_In_elements.
+    - eapply Clauses_In_elements in H0. apply add_clause_inj in H. now subst.
+  Qed.
+
+  Lemma in_add_clauses {cl cls} n : Clauses.In cl (add_clauses n cls) -> exists cl', Clauses.In cl' cls /\ cl = add_clause n cl'.
+  Proof.
+    unfold succ_clauses.
+    rewrite ClausesProp.of_list_1 InA_In_eq in_map_iff.
+    firstorder eauto.
+    exists x; split => //. unfold ClausesProp.to_list. now eapply Clauses_In_elements.
+  Qed.
+
+  Lemma clauses_levels_add {n cls} : clauses_levels (add_clauses n cls) =_lset clauses_levels cls.
+  Proof.
+    intros l.
+    rewrite clauses_levels_spec.
+    split.
+    - move=> [] cl [] /in_add_clauses [] cl' [] incl' ->.
+      rewrite clause_levels_spec. cbn. destruct cl; cbn.
+      intros h. apply clauses_levels_spec. exists cl'; split => //.
+      move: h; case.
+      move/levelexprset_levels_spec => [k].
+      destruct cl'; cbn in * => /In_add_prems => [] [] x [].
+      destruct x => hin [=] ->. intros ->.
+      apply clause_levels_spec. left. apply levelexprset_levels_spec. now exists z.
+      intros ->. apply clause_levels_spec; right. destruct cl' => //=. destruct t0 => //.
+    - move/clauses_levels_spec => [] cl [] hin /clause_levels_spec [].
+      * move=> /levelexprset_levels_spec => [] [k hin']; exists (add_clause n cl); split => //.
+        now apply add_clauses_spec.
+        apply clause_levels_spec. left.
+        apply levelexprset_levels_spec. exists (k + n).
+        destruct cl; cbn. apply In_add_prems. exists (l, k).
+        split => //.
+      * intros ->. exists (add_clause n cl); split => //. now apply add_clauses_spec.
+        apply clause_levels_spec. right.
+        destruct cl; cbn. destruct t => //.
+  Qed.
+
+  Lemma add_clause_0 cl : add_clause 0 cl = cl.
+  Proof.
+    destruct cl as [prems [concl k]]; cbn.
+    f_equal. 2:now rewrite Z.add_0_r.
+    unfold add_prems.
+    eapply eq_univ_equal. intros [l k'].
+    rewrite NonEmptySetFacts.map_spec.
+    unfold add_expr. split.
+    - intros [[] [hin heq]]. noconf heq. now rewrite Z.add_0_r.
+    - exists (l, k'); split => //. now rewrite Z.add_0_r.
+  Qed.
+
+  Variant in_pred_closure cls : clause -> Prop :=
+  | incls cl n : Clauses.In cl cls -> in_pred_closure cls (add_clause n cl)
+  | predcl x k : in_pred_closure cls (singleton (x, k + 1), (x, k)).
+  Derive Signature for in_pred_closure.
+
+  Inductive entails (cls : clauses) : clause -> Prop :=
+  | clause_in (prems : premises) (concl : LevelExpr.t) :
+    LevelExprSet.In concl prems -> entails cls (prems, concl)
+  | clause_cut prems' concl' prems concl :
+    in_pred_closure cls (prems', concl') ->
+    entails cls (add concl' prems, concl) ->
+    LevelExprSet.Subset prems' prems ->
+    entails cls (prems, concl).
+
+  Definition entails_all cls (prems concls : premises) :=
+    LevelExprSet.For_all (fun le => entails cls (prems, le)) concls.
+
+  Notation " cls ⊢ prems → concl " := (entails cls (prems, concl)) (at level 20).
+  Notation " cls ⊢a prems → concl " := (entails_all cls prems concl) (at level 20).
+
+  Lemma in_pred_closure_equal cls (prems prems' : premises) concl :
+    LevelExprSet.Equal prems prems' ->
+    in_pred_closure cls (prems, concl) -> in_pred_closure cls (prems', concl).
+  Proof.
+    intros eq. apply NonEmptySetFacts.eq_univ_equal in eq. now subst prems.
+  Qed.
+
+  Lemma entails_equal cls (prems prems' : premises) concl :
+    LevelExprSet.Equal prems prems' ->
+    entails cls (prems, concl) -> entails cls (prems', concl).
+  Proof.
+    intros he en.
+    replace prems' with prems => //.
+    now apply eq_univ_equal.
+  Qed.
+
+  Lemma entails_plus cls c : entails cls c -> entails (succ_clauses cls) (succ_clause c).
+  Proof.
+    induction 1.
+    - constructor. apply map_spec. exists concl0. split => //.
+    - eapply clause_cut with (succ_prems prems') (succ_expr concl').
+      + depelim H.
+        * have -> : (succ_prems prems', succ_expr concl') = add_clause n (succ_clause cl).
+          { destruct cl as [prems'' concl'']. cbn in H0. noconf H0.
+            rewrite add_prems_add_prems add_expr_add_expr add_clause_add_clause.
+            now rewrite Z.add_1_r Z.add_1_l. }
+          constructor. now rewrite -add_clauses_spec.
+        * have eq : (succ_prems (singleton (x, (k + 1)))) = (singleton (x, k + 1 + 1)).
+          { apply eq_univ_equal. unfold succ_prems.
+            intros le. rewrite map_spec LevelExprSet.singleton_spec.
+            split.
+            { intros [? [hin ->]].
+              rewrite LevelExprSet.singleton_spec in hin. red in hin; subst x0.
+              reflexivity. }
+            { unfold LevelExprSet.E.eq. intros ->.
+              exists (x, k + 1). split.
+              now rewrite LevelExprSet.singleton_spec. reflexivity. } }
+          rewrite eq. constructor 2.
+      + unfold succ_clause in IHentails.
+        eapply entails_equal; tea.
+        intros x. rewrite /succ_prems. rewrite map_spec add_spec.
+        setoid_rewrite add_spec. rewrite map_spec.
+        firstorder eauto. subst. now left.
+      + intros x. rewrite /succ_prems !map_spec.
+        intros [e [hin ->]]. exists e. firstorder.
+  Qed.
+
+
+  Derive Signature for entails.
+
+  Lemma entails_pred_closure {cls prems concl k} :
+    cls ⊢ prems → (concl, 1 + k) -> cls ⊢ prems → (concl, k).
+  Proof.
+    intros he.
+    Opaque Z.add.
+    depind he.
+    - eapply clause_cut.
+      constructor.
+      2:{ intros l hin. rewrite LevelExprSet.singleton_spec in hin. red in hin; subst l.
+          rewrite Z.add_comm; exact H. }
+      constructor.
+      rewrite LevelExprSet.add_spec. lesets.
+    - eapply clause_cut; tea.
+  Qed.
+
+  Lemma entails_pred_closure_n {cls prems concl k n} :
+    entails cls (prems, (concl, k + Z.of_nat n)) -> entails cls (prems, (concl, k)).
+  Proof.
+    induction n in k |- *.
+    - rewrite Z.add_0_r. tauto.
+    - intros hen. rewrite Nat2Z.inj_succ in hen. rewrite Z.add_succ_r in hen.
+      eapply IHn. move: hen.
+      have -> : Z.succ (k + Z.of_nat n) = 1 + (k + Z.of_nat n) by lia.
+      eapply entails_pred_closure.
+  Qed.
+
+
+  Lemma incls0 {cls cl} : Clauses.In cl cls -> in_pred_closure cls cl.
+  Proof.
+    intros hin.
+    have hcl := incls _ _ 0 hin.
+    now rewrite add_clause_0 in hcl.
+  Qed.
+
+  Lemma entails_in {cls cl} : Clauses.In cl cls -> entails cls cl.
+  Proof.
+    intros hin.
+    destruct cl as [prems concl].
+    eapply clause_cut.
+    - now eapply incls0.
+    - constructor. eapply LevelExprSet.add_spec. now left.
+    - reflexivity.
+  Qed.
+
+  Lemma in_pred_closure_shift {cls cl} n : in_pred_closure cls cl -> in_pred_closure cls (add_clause n cl).
+  Proof.
+    destruct 1.
+    - rewrite add_clause_add_clause. now constructor.
+    - cbn. eapply in_pred_closure_equal with (singleton (x, k + 1 + n)).
+      { intros le. rewrite In_add_prems; rewrite_strat (topdown LevelExprSet.singleton_spec).
+        intuition auto. exists (x, k + 1). split => //.
+        now destruct H as [le' [-> ->]]. }
+      have -> : k + 1 + n = (k + n) + 1 by lia.
+      constructor.
+  Qed.
+
+  Lemma add_clause_singleton n le concl k : add_clause n (singleton le, (concl, k)) = (singleton (add_expr n le), (concl, k + n)).
+  Proof.
+    rewrite /add_clause //=. f_equal.
+    apply eq_univ_equal. intros le'. rewrite In_add_prems.
+    rewrite_strat (topdown LevelExprSet.singleton_spec).
+    unfold LevelExprSet.E.eq. firstorder. subst. reflexivity.
+  Qed.
+
+  Lemma entails_shift {cls cl} n : entails cls cl -> entails cls (add_clause n cl).
+  Proof.
+    induction 1.
+    - unfold add_clause. constructor.
+      rewrite In_add_prems. exists concl0. split => //.
+    - eapply (clause_cut _ (add_prems n prems') (add_expr n concl')).
+      2:{ unfold add_clause in *. eapply entails_equal; tea.
+      intros le. setoid_rewrite In_add_prems. setoid_rewrite LevelExprSet.add_spec.
+      setoid_rewrite In_add_prems.
+      unfold LevelExprSet.E.eq. firstorder. subst. now left. }
+      2:{ intros x. rewrite !In_add_prems. firstorder. }
+      eapply (in_pred_closure_shift _ H).
+  Qed.
+
+  Lemma entails_subset cls (prems prems' : premises) concl : LevelExprSet.Subset prems prems' ->
+    entails cls (prems, concl) ->
+    entails cls (prems', concl).
+  Proof.
+    intros hsubt.
+    intros H; revert prems' hsubt; depind H.
+    - constructor. eapply hsubt, H.
+    - intros prems'' hsub.
+      eapply clause_cut. 2:eapply IHentails. tea.
+      2:lesets. intros x; rewrite !LevelExprSet.add_spec. firstorder.
+  Qed.
+
+  Lemma entails_trans {cls prems concl concl'} :
+    entails cls (prems, concl) ->
+    entails cls (singleton concl, concl') ->
+    entails cls (prems, concl').
+  Proof.
+    intros H; depind H.
+    - intros he.
+      depelim he.
+      * rewrite LevelExprSet.singleton_spec in H0. red in H0; subst concl0.
+        now constructor.
+      * eapply (clause_cut _ prems'). tea.
+        eapply entails_subset; tea.
+        intros ?; rewrite !LevelExprSet.add_spec LevelExprSet.singleton_spec; firstorder.
+        red in H2; subst a. now right. intros x. firstorder. apply H1 in H2.
+        rewrite LevelExprSet.singleton_spec in H2. now red in H2; subst x.
+    - intros he.
+      specialize (IHentails concl'0 he).
+      eapply clause_cut; tea.
+  Qed.
+
+  Lemma entails_weak {cls prem concl concl'} :
+    entails cls (prem, concl) ->
+    entails cls (add concl' prem, concl).
+  Proof.
+    intros H. depind H.
+    - constructor. apply LevelExprSet.add_spec. now right.
+    - eapply (clause_cut _ _ concl'); tea.
+      rewrite add_comm. apply IHentails.
+      intros x; rewrite LevelExprSet.add_spec. firstorder.
+  Qed.
+
+  Lemma entails_weak_union {cls prem concl concl'} :
+    entails cls (prem, concl) ->
+    entails cls (univ_union concl' prem, concl).
+  Proof.
+    intros hyp.
+    move: concl'.
+    apply: premises_elim.
+    - intros le. rewrite univ_union_comm univ_union_add_singleton.
+      now apply entails_weak.
+    - intros le prems ih.
+      rewrite univ_union_add_distr. intros _.
+      now eapply entails_weak.
+  Qed.
+
+  Lemma entails_all_weak {cls prem concl concl'} :
+    entails_all cls prem concl ->
+    entails_all cls (add concl' prem) concl.
+  Proof.
+    intros hcl x hin.
+    specialize (hcl _ hin). cbn in hcl.
+    now apply entails_weak.
+  Qed.
+
+  Lemma entails_all_weak_union {cls prem concl concl'} :
+    entails_all cls prem concl ->
+    entails_all cls (univ_union concl' prem) concl.
+  Proof.
+    intros hcl x hin.
+    specialize (hcl _ hin). cbn in hcl.
+    now apply entails_weak_union.
+  Qed.
+
+  Lemma entails_all_weak' {cls prem concl concl'} :
+    entails_all cls prem concl ->
+    entails_all cls (add concl' prem) (add concl' concl).
+  Proof.
+    intros hcl x hin.
+    eapply LevelExprSet.add_spec in hin as []. red in H; subst.
+    - constructor. eapply LevelExprSet.add_spec. now left.
+    - specialize (hcl _ H). cbn in hcl.
+      now apply entails_weak.
+  Qed.
+
+  Lemma entails_cut_all {cls prems' concl' prems concls} :
+    in_pred_closure cls (prems', concl') ->
+    cls ⊢a add concl' prems → concls ->
+    prems' ⊂_leset prems ->
+    cls ⊢a prems → concls.
+  Proof.
+    intros inp he hp x hin.
+    eapply clause_cut; tea.
+    now apply he in hin.
+  Qed.
+
+  Lemma entails_all_subset {cls} {prems prems' prems'' : premises} :
+    prems'' ⊂_leset prems' ->
+    cls ⊢a prems → prems' ->
+    cls ⊢a prems → prems''.
+  Proof.
+    intros incl ha x hin.
+    eapply incl in hin. now apply ha in hin.
+  Qed.
+
+  Lemma entails_all_add cls prem l prems' :
+    cls ⊢a prem → add l prems' <->
+    cls ⊢ prem → l /\ cls ⊢a prem → prems'.
+  Proof.
+    rewrite /entails_all /LevelExprSet.For_all.
+    setoid_rewrite LevelExprSet.add_spec; rewrite /LevelExprSet.E.eq.
+    firstorder. now subst.
+  Qed.
+
+  Lemma entails_add {cls prems cl concl} :
+    entails cls (prems, cl) ->
+    entails cls (add cl prems, concl) ->
+    entails cls (prems, concl).
+  Proof.
+    intros H; depind H.
+    - intros he.
+      depelim he.
+      * rewrite LevelExprSet.add_spec in H0. destruct H0 as [].
+        { red in H0; subst concl0. now constructor. }
+        { now constructor. }
+      * have eq : prems = add concl0 prems.
+        { eapply eq_univ_equal. intros x; rewrite LevelExprSet.add_spec. firstorder. now red in H2; subst. }
+        rewrite -eq in H1.
+        eapply (clause_cut _ prems' _ prems). tea. 2:tea.
+        now rewrite -eq in he.
+    - intros he.
+      eapply clause_cut. tea. eapply IHentails.
+      rewrite add_comm. now eapply entails_weak.
+      exact H1.
+  Qed.
+
+  Lemma entails_cumul_one {cls prems prems' concl} :
+    entails_all cls prems prems' ->
+    entails cls (univ_union prems prems', concl) ->
+    entails cls (prems, concl).
+  Proof.
+    revert prems' prems concl.
+    apply: premises_elim.
+    - intros. specialize (H le). forward H by now apply LevelExprSet.singleton_spec.
+      cbn in H.
+      eapply entails_add; tea.
+      now rewrite -univ_union_add_singleton.
+    - intros le prems ih _ prem concl' hadd hadd'.
+      rewrite univ_union_comm univ_union_add_distr -univ_union_comm -univ_union_add_distr in hadd'.
+      eapply ih in hadd'. 2:{ apply entails_all_weak. apply entails_all_add in hadd as []. exact H0. }
+      apply entails_all_add in hadd as [].
+      eapply entails_add; tea.
+  Qed.
+
+  Lemma entails_all_cumul {cls prems prems' concl} :
+    entails_all cls prems prems' ->
+    entails_all cls (univ_union prems prems') concl ->
+    entails_all cls prems concl.
+  Proof.
+    intros hp hc.
+    intros x hin. apply hc in hin.
+    eapply entails_cumul_one; tea.
+  Qed.
+
+  Lemma entails_all_one {cls prem concl concl'} :
+    entails_all cls prem concl ->
+    entails cls (concl, concl') ->
+    entails cls (prem, concl').
+  Proof.
+    intros ha he.
+    eapply entails_cumul_one; tea.
+    now eapply entails_weak_union.
+  Qed.
+
+  Lemma entails_all_trans {cls prem concl concl'} :
+    entails_all cls prem concl ->
+    entails_all cls concl concl' ->
+    entails_all cls prem concl'.
+  Proof.
+    intros ha he cl hin.
+    apply he in hin.
+    eapply entails_all_one; tea.
+  Qed.
+
+  Lemma entails_incr_shift cls concl k n :
+    entails cls (singleton (concl, k), (concl, k + 1)) ->
+    entails cls (singleton (concl, k), (concl, k + 1 + Z.of_nat n)).
+  Proof.
+    induction n in k |- *; auto.
+    - now rewrite Z.add_0_r.
+    - intros en.
+      have hs := entails_shift 1 en. rewrite add_clause_singleton /= in hs.
+      apply IHn in hs.
+      eapply entails_trans; tea.
+      now have -> : k + 1 + Z.of_nat (S n) = k + 1 + 1 + Z.of_nat n by lia.
+  Qed.
+
+  Lemma entails_incr_all cls concl k :
+    entails cls (singleton (concl, k), (concl, k + 1)) ->
+    forall k', entails cls (singleton (concl, k), (concl, k')).
+  Proof.
+    intros en k'.
+    destruct (Z.lt_trichotomy k k') as [|[]]; subst; auto.
+    - have ispos : 0 <= k' - k - 1 by lia.
+      eapply (entails_incr_shift _ _ _ (Z.to_nat (k' - k - 1))) in en.
+      assert (k + 1 + Z.of_nat (Z.to_nat (k' - k - 1)) = k') by lia. now rewrite H0 in en.
+    - constructor. now rewrite LevelExprSet.singleton_spec.
+    - have [k0 ->] : (exists kd : nat, k = k' + Z.of_nat kd). { exists (Z.to_nat (k - k')). lia. }
+      eapply (entails_pred_closure_n (n:=k0)). constructor. now apply LevelExprSet.singleton_spec.
+  Qed.
+
+  Lemma entails_all_concl_union {cls prems concl concl'} :
+    cls ⊢a prems → concl ->
+    cls ⊢a prems → concl' ->
+    cls ⊢a prems → univ_union concl concl'.
+  Proof.
+    intros l r.
+    rewrite /entails_all.
+    intros x. rewrite univ_union_spec. intros []. now apply l. now apply r.
+  Qed.
+
+  Lemma entails_all_union {cls prems concl prems' concl'} :
+    cls ⊢a prems → concl ->
+    cls ⊢a prems' → concl' ->
+    cls ⊢a univ_union prems prems' → univ_union concl concl'.
+  Proof.
+    intros l r.
+    apply entails_all_concl_union.
+    rewrite univ_union_comm.
+    now eapply entails_all_weak_union.
+    now eapply entails_all_weak_union.
+  Qed.
+
+
+  Lemma entails_all_shift {cls : clauses} {prems concl : premises} (n : Z) :
+    cls ⊢a prems → concl ->
+    cls ⊢a add_prems n prems → add_prems n concl.
+  Proof.
+    intros cla cl.
+    rewrite In_add_prems => [[le' [hin ->]]].
+    eapply (entails_shift (cl := (prems, le'))).
+    now apply cla in hin.
+  Qed.
+
+  Lemma in_pred_closure_subset {cls cls' prems concl} :
+    in_pred_closure cls (prems, concl) ->
+    cls ⊂_clset cls' ->
+    in_pred_closure cls' (prems, concl).
+  Proof.
+    induction 1.
+    - move/(_ _ H). now constructor.
+    - constructor.
+  Qed.
+
+  Lemma entails_clauses_subset cls cls' prems concl :
+    cls ⊢ prems → concl ->
+    cls ⊂_clset cls' ->
+    cls' ⊢ prems → concl.
+  Proof.
+    induction 1 in cls' |- * => incl.
+    - now constructor.
+    - eapply clause_cut.
+      + eapply in_pred_closure_subset; tea.
+      + now apply IHentails.
+      + assumption.
+  Qed.
+
+  Lemma entails_all_clauses_subset cls cls' prems concl :
+    cls ⊢a prems → concl ->
+    cls ⊂_clset cls' ->
+    cls' ⊢a prems → concl.
+  Proof.
+    intros d incl [l k].
+    now move/d/entails_clauses_subset.
+  Qed.
+
+  Lemma entails_succ cls (u v : premises) :
+    (forall l k, LevelExprSet.In (l, k) v -> exists k', LevelExprSet.In (l, k') u /\ k <= k') ->
+    cls ⊢a u → v.
+  Proof.
+    intros hk [l k] hin.
+    specialize (hk _ _ hin) as [k' [hin' le]].
+    assert (exists n, k' = k + n) as [n ->] by (exists (k' - k); lia).
+    eapply (entails_pred_closure_n (n := Z.to_nat n)).
+    constructor. rewrite Z2Nat.id. lia. assumption.
+  Qed.
+
+  Lemma entails_all_tauto cls u : cls ⊢a u → u.
+  Proof.
+    intros x hin. now constructor.
+  Qed.
+
+  Lemma loop_any_successor cls u n :
+    cls ⊢a u → succ_prems u ->
+    cls ⊢a u → add_prems (Z.of_nat (S n)) u.
+  Proof.
+    induction n.
+    - auto.
+    - intros ass.
+      specialize (IHn ass).
+      have sh := entails_all_shift 1 IHn.
+      eapply entails_all_trans. tea.
+      rewrite add_prems_add_prems in sh.
+      have eq : 1 + Z.of_nat (S n) = Z.of_nat (S (S n)) by lia.
+      now rewrite eq in sh.
+  Qed.
+
+  Lemma entails_pred_closure_neg {cls u concl k p} :
+    cls ⊢ u → (concl, k) ->
+    cls ⊢ u → (concl, k + Z.neg p).
+  Proof.
+    intros ent.
+    eapply (entails_pred_closure_n (n := Pos.to_nat p)).
+    have eq : Z.neg p + Z.of_nat (Pos.to_nat p) = 0. lia.
+    now rewrite -Z.add_assoc eq Z.add_0_r.
+  Qed.
+
+  Lemma loop_any cls u n :
+    cls ⊢a u → succ_prems u ->
+    cls ⊢a u → add_prems n u.
+  Proof.
+    destruct n.
+    - rewrite add_prems_0. intros _. apply entails_all_tauto.
+    - assert (exists n, Z.pos p = Z.of_nat n). exists (Pos.to_nat p). now rewrite Z_of_pos_alt.
+      destruct H as [n ->]. destruct n. cbn. intros. rewrite add_prems_0. apply entails_all_tauto.
+      apply loop_any_successor.
+    - intros _ [l k]. rewrite In_add_prems.
+      intros [[] [hin heq]]. rewrite /add_expr in heq. noconf heq.
+      apply entails_pred_closure_neg.
+      now constructor.
+  Qed.
 
 End Clauses.
