common/theories/LoopChecking/Deciders.v
@@ -1,0 +1,2027 @@
+(* Distributed under the terms of the MIT license. *)
+From Stdlib Require Import ssreflect ssrbool ZArith.
+From Stdlib Require Import Program RelationClasses Morphisms.
+From Stdlib Require Import Orders OrderedTypeAlt OrderedTypeEx MSetList MSetInterface MSetAVL MSetFacts FMapInterface MSetProperties MSetDecide.
+From MetaRocq.Utils Require Import utils.
+
+From MetaRocq.Common Require Universes.
+From Equations Require Import Equations.
+
+From MetaRocq.Common.LoopChecking Require Import Common Interfaces HornClauses Model PartialLoopChecking.
+
+Set Equations Transparent.
+
+Module Type LoopCheckingItf (LS : LevelSets).
+
+  (* Type of consistent models of a set of universe constraints *)
+  Parameter model : Type.
+  Notation univ := LS.LevelExprSet.nonEmptyLevelExprSet.
+
+  Inductive constraint_type := UnivEq | UnivLe.
+  Notation constraint := (univ * constraint_type * univ).
+
+  Parameter init_model : model.
+
+  (* Returns None if already declared *)
+  Parameter declare_level : LS.Level.t -> model -> option model.
+
+  (* If the constraints mention undeclared universes, returns None,
+     otherwise, returns either a model or a looping universe, i.e. such that u >= u + 1 is implied
+     by the constraint *)
+  Parameter enforce : constraint -> model -> option (model + univ).
+
+  (* Returns true is the clause is valid in the model and all its possible consistent extensions.
+     Returns false if the constraint results in an inconsistent set of constraints or it simply
+     is not valid. *)
+  Parameter check : model -> constraint -> bool.
+
+  (* Returns the valuation of the model: a minimal assignement from levels to constraints
+    that make the enforced clauses valid. *)
+  Parameter valuation : model -> LS.LevelMap.t nat.
+End LoopCheckingItf.
+
+Module Deciders (LS : LevelSets).
+
+Module Import I := LoopCheckingImpl LS.
+Import LS.
+
+Local Open Scope Z_scope.
+
+Definition init_model cls := max_clause_premises cls.
+
+Lemma init_model_levels cls k :
+  LevelMap.In k (init_model cls) <-> LevelSet.In k (clauses_levels cls).
+Proof.
+  split.
+  - now move => [] k' /max_clause_premises_spec.
+  - move/max_clause_premises_spec_inv. now eexists.
+Qed.
+
+Definition init_w (levels : LevelSet.t) : LevelSet.t := LevelSet.empty.
+
+(* We don't need predecessor clauses as they are trivially satisfied *)
+(* Definition add_predecessors (V : LevelSet.t) cls :=
+  LevelSet.fold (fun l acc =>
+    Clauses.add (NonEmptySetFacts.singleton (l, 1), (l, 0)) acc) V cls. *)
+
+Definition infer_result V cls := result V LevelSet.empty cls (init_model cls).
+
+Equations? infer (cls : clauses) : infer_result (clauses_levels cls) cls :=
+  infer cls := loop (clauses_levels cls) LevelSet.empty cls (init_model cls) (init_model cls) (And3 _ _ _).
+Proof.
+  - now rewrite -init_model_levels.
+  - apply is_update_of_empty.
+Qed.
+
+Local Open Scope string_scope2.
+
+Definition print_level_Z_map (m : LevelMap.t (option Z)) :=
+  let list := LevelMap.elements m in
+  print_list (fun '(l, w) => Level.to_string l ^ " -> " ^ string_of_option string_of_Z w) nl list.
+
+Definition print_result {V cls} (m : infer_result V cls) :=
+  match m return string with
+  | Loop _ _ => "looping on "
+  | Model w m _ => "satisfiable with model: " ^ print_level_Z_map m.(model_model) ^ nl ^ " W = " ^
+    print_lset w
+    ^ nl ^ "valuation: " ^ print_level_nat_map (valuation_of_model m.(model_model))
+  end.
+
+Definition valuation_of_result {V cls} (m : infer_result V cls) :=
+  match m with
+  | Loop _ _  => "looping"
+  | Model w m _ => print_level_nat_map (valuation_of_model m.(model_model))
+  end.
+
+Definition to_string_expr (e : LevelExpr.t) : string :=
+  let '(l, n) := e in Level.to_string l ^ (if n is Z0 then "" else "+" ^ string_of_Z n).
+
+Definition print_premise (l : premises) : string :=
+  let (e, exprs) := NonEmptySetFacts.to_nonempty_list l in
+  to_string_expr e ^
+  match exprs with
+  | [] => ""
+  | _ => ", " ^ print_list to_string_expr ", " exprs
+  end.
+
+Definition print_clauses (cls : clauses) :=
+  let list := Clauses.elements cls in
+  print_list (fun '(l, r) =>
+    print_premise l ^ " → " ^ to_string_expr r) nl list.
+
+Definition valuation := LevelMap.t nat.
+
+Equations? infer_model (cls : clauses) : option model :=
+infer_model cls with loop (clauses_levels cls) LevelSet.empty cls (init_model cls) (init_model cls) _ :=
+  | Loop _ _ => None
+  | Model w vm heq => Some vm.(model_model).
+Proof.
+  split.
+  - reflexivity.
+  - apply infer_obligation_2.
+  - apply is_update_of_empty.
+Qed.
+
+Definition enabled_clause (m : model) (cl : clause) :=
+  exists z, min_premise m (premise cl) = Some z.
+
+Definition enabled_clauses (m : model) (cls : clauses) :=
+  Clauses.For_all (enabled_clause m) cls.
+
+Definition correct_model (cls : clauses) (m : model) :=
+  enabled_clauses m cls /\ clauses_sem (valuation_of_model m) cls.
+
+Definition infer_correctness cls :=
+  match infer_model cls with
+  | Some m => correct_model cls m
+  | None => ~ exists v, clauses_sem v cls
+  end.
+
+Lemma enabled_clauses_ext m m' cls : m ⩽ m' -> enabled_clauses m cls -> enabled_clauses m' cls.
+Proof.
+  intros hext.
+  rewrite /enabled_clauses.
+  intros ha cl; move/ha.
+  unfold enabled_clause.
+  intros [minp heq].
+  have hp := min_premise_pres (premise cl) hext.
+  rewrite heq in hp. depelim hp. now exists y.
+Qed.
+
+Lemma interp_prems_ge v (prems : premises) :
+  forall prem, LevelExprSet.In prem prems ->
+  interp_expr v prem <= interp_prems v prems.
+Proof.
+  intros.
+  unfold interp_prems.
+  have he := to_nonempty_list_spec prems.
+  destruct to_nonempty_list.
+  pose proof to_nonempty_list_spec'.
+  rewrite In_elements in H. rewrite -he in H. clear H0 he. clear -H.
+  destruct H. subst p.
+  - induction l. cbn. auto.
+    cbn. lia. cbn. lia.
+  - induction l in H |- *.
+    now cbn in H.
+    cbn in H. destruct H; subst; cbn.
+    * cbn. lia.
+    * specialize (IHl H). lia.
+Qed.
+
+(** Enabled and valid clauses are satisfied by valuation *)
+Lemma valid_clause_model model cl :
+  enabled_clause model cl ->
+  valid_clause model cl ->
+  clause_sem (valuation_of_model model) cl.
+Proof.
+  unfold enabled_clause, valid_clause.
+  destruct min_premise eqn:hmin => //= => //.
+  2:{ intros [k' eq]. congruence. }
+  intros [k' eq]. noconf eq.
+  destruct cl as [prems [concl k]]; cbn.
+  unfold level_value_above.
+  destruct level_value eqn:hl => //.
+  unfold interp_level. unfold level_value in hl. destruct LevelMap.find eqn:hfind => //. noconf hl.
+  move/Z.leb_le => hrel.
+  eapply LevelMap.find_2 in hfind.
+  have conclm := valuation_of_model_spec _ _ _ hfind.
+  set (v := (model_max _ - _)) in *.
+  cbn in conclm.
+  eapply LevelMap.find_1 in conclm. rewrite conclm.
+  subst v.
+  pose proof (@min_premise_spec model prems) as [premmin [prem [premin premeq]]].
+  rewrite hmin in premeq.
+  eapply Z.le_ge.
+  eapply Z.le_trans. 2:{ eapply interp_prems_ge; tea. }
+  unfold interp_expr. destruct prem as [prem k'].
+  symmetry in premeq.
+  move: premeq. unfold min_atom_value.
+  unfold level_value. destruct (LevelMap.find prem) eqn:findp => //.
+  destruct o => //.
+  intros [= <-].
+  eapply LevelMap.find_2 in findp.
+  have premm := valuation_of_model_spec _ _ _ findp.
+  unfold interp_level.
+  eapply LevelMap.find_1 in premm. rewrite premm.
+  assert (z1 - k' <= z0 - k). lia.
+  have hm : z0 <= model_max model.
+  { eapply model_max_spec in hfind; tea. now depelim hfind. }
+  have hm' : z1 <= model_max model.
+  { eapply model_max_spec in findp; tea. now depelim findp. }
+  have hmi : model_min model <= z0.
+  { eapply model_min_spec; tea. }
+  have hmi' : model_min model <= z1.
+  { eapply model_min_spec; tea. }
+  assert (0 <= model_max model)%Z by apply model_max_spec2.
+  assert (model_min model <= 0)%Z by apply model_min_spec2.
+  lia.
+Qed.
+
+Lemma init_model_enabled cls : enabled_clauses (init_model cls) cls.
+Proof.
+  unfold enabled_clauses.
+  intros x hin. unfold enabled_clause.
+  pose proof (@min_premise_spec (init_model cls) (premise x)) as [premmin [prem [premin premeq]]].
+  have inV : LevelSet.In prem (clauses_levels cls).
+  { rewrite clauses_levels_spec. exists x; split => //. rewrite /clause_levels.
+    eapply LevelSet.union_spec; left. rewrite levelexprset_levels_spec. exists prem.2.
+    destruct prem. exact premin. }
+  unfold init_model. rewrite premeq. unfold min_atom_value.
+  destruct prem as [l k].
+  have hm := max_clause_premises_spec_inv cls l inV.
+  rewrite (level_value_MapsTo hm).
+  have hs := max_clause_premise_of_spec l k _ _ hin premin.
+  depelim hs. rewrite H0.
+  eexists => //.
+Qed.
+
+Lemma interp_add_expr V n e : interp_expr V (add_expr n e) = n + interp_expr V e.
+Proof.
+  destruct e as [l k]; cbn. lia.
+Qed.
+
+Lemma interp_prems_singleton V e :
+  interp_prems V (singleton e) = interp_expr V e.
+Proof.
+  rewrite /interp_prems.
+  now rewrite singleton_to_nonempty_list /=.
+Qed.
+
+Lemma fold_right_max_in {a l} n : In a l -> a <= fold_right Z.max n l.
+Proof.
+  induction l.
+  - now cbn.
+  - intros [eq|inl]. subst a0. cbn. lia.
+    cbn. specialize (IHl inl). lia.
+Qed.
+
+Lemma fold_right_max_acc {n l} : n <= fold_right Z.max n l.
+Proof.
+  induction l.
+  - now cbn.
+  - cbn. lia.
+Qed.
+
+Lemma fold_right_impl n l l' :
+  (forall x, In x l -> In x l') -> fold_right Z.max n l <= fold_right Z.max n l'.
+Proof.
+  induction l in l' |- *.
+  - cbn. destruct l'; cbn. lia.
+    intros. have := @fold_right_max_acc n l'. lia.
+  - cbn; intros h.
+    have inal' := (h a (or_introl eq_refl)).
+    have := fold_right_max_in n inal'.
+    specialize (IHl l').
+    forward IHl.
+    intros. apply h. now right.
+    lia.
+Qed.
+
+Lemma fold_right_equivlist n l l' :
+  equivlistA eq l l' -> fold_right Z.max n l = fold_right Z.max n l'.
+Proof.
+  intros eq.
+  have h := fold_right_impl n l l'.
+  forward h. intros x; rewrite -!InA_In_eq. apply eq.
+  have h' := fold_right_impl n l' l.
+  forward h'. intros x; rewrite -!InA_In_eq. apply eq.
+  lia.
+Qed.
+
+Fixpoint max_list (l : list Z) : option Z :=
+  match l with
+  | [] => None
+  | x :: xs => match max_list xs with
+    | Some m => Some (Z.max x m)
+    | None => Some x end
+  end.
+
+Lemma max_list_fold_right n l : max_list (n :: l) = Some (fold_right Z.max n l).
+Proof.
+  induction l; cbn.
+  - reflexivity.
+  - cbn in IHl. destruct max_list. f_equal. noconf IHl. lia.
+    f_equal; noconf IHl. lia.
+Qed.
+
+Lemma fold_right_max_spec n l :
+  let fn := fold_right Z.max in
+  (forall x, In x (n :: l) -> x <= fn n l) /\
+  (exists x, In x (n :: l) /\ fn n l = x).
+Proof.
+  induction l; cbn.
+  - split. intros x [] => //. now subst.
+    exists n. firstorder.
+  - cbn in IHl. destruct IHl as [h h'].
+    split.
+    intros x [|[]]; subst.
+    * specialize (h x). forward h by auto. lia.
+    * lia.
+    * specialize (h x). forward h by auto. lia.
+    * destruct h' as [x []]. exists (Z.max a x). rewrite -{4}H0. split => //.
+      destruct H; subst.
+      destruct (Z.max_spec a x) as [[]|[]]; firstorder; subst.
+      destruct (Z.max_spec a (fold_right Z.max n l)) as [[]|[]]; firstorder; subst. rewrite H1.
+      auto.
+Qed.
+
+Lemma fold_right_equivlist_all n n' l l' :
+  equivlistA eq (n :: l) (n' :: l') -> fold_right Z.max n l = fold_right Z.max n' l'.
+Proof.
+  intros eq.
+  have [hla [maxl [inmaxl eqmaxl]]] := fold_right_max_spec n l.
+  have [hra [maxr [inmaxr eqmaxr]]] := fold_right_max_spec n' l'.
+  rewrite eqmaxl eqmaxr.
+  red in eq; setoid_rewrite InA_In_eq in eq.
+  apply (eq _) in inmaxl. apply hra in inmaxl.
+  apply eq in inmaxr. apply hla in inmaxr. lia.
+Qed.
+
+Lemma interp_prems_elements V u :
+  interp_prems V u = fold_right Z.max (interp_expr V (to_nonempty_list u).1) (List.map (interp_expr V) (to_nonempty_list u).2).
+Proof.
+  rewrite /interp_prems.
+  have he := to_nonempty_list_spec u.
+  destruct to_nonempty_list.
+  now rewrite Universes.fold_right_map.
+Qed.
+
+Lemma fold_right_interp {V x l x' l'} :
+  equivlistA eq (x :: l) (x' :: l') ->
+  fold_right Z.max (interp_expr V x) (List.map (interp_expr V) l) = fold_right Z.max (interp_expr V x') (List.map (interp_expr V) l').
+Proof.
+  intros eq. apply fold_right_equivlist_all.
+  intros a. rewrite !InA_In_eq.
+  rewrite !(in_map_iff (interp_expr V) (_ :: _)).
+  setoid_rewrite <-InA_In_eq.
+  split.
+  - move=> [b [<- ]].
+    eexists; split; trea. now apply eq in b0.
+  - move=> [b [<- ]].
+    eexists; split; trea. now apply eq in b0.
+Qed.
+
+Lemma equivlistA_add le u : let l := to_nonempty_list (add le u) in
+ equivlistA eq (l.1 :: l.2) (le :: LevelExprSet.elements u).
+Proof.
+  have he := to_nonempty_list_spec (add le u).
+  destruct to_nonempty_list. cbn.
+  intros x. rewrite he.
+  rewrite !LevelExprSet.elements_spec1.
+  split.
+  - move/LevelExprSet.add_spec => [->|hin].
+    now constructor. constructor 2. now apply LevelExprSet.elements_spec1.
+  - intros h; depelim h; subst. now apply LevelExprSet.add_spec; left.
+    apply LevelExprSet.add_spec. now apply LevelExprSet.elements_spec1 in h.
+Qed.
+
+Lemma fold_right_comm acc l : l <> [] -> fold_right Z.max acc l = Z.max acc (fold_right Z.max (List.hd acc l) (List.tl l)).
+Proof.
+  induction l in acc |- *.
+  - intros; congruence.
+  - intros _. cbn. destruct l; cbn. lia.
+    cbn in IHl. rewrite (IHl acc). congruence.
+    rewrite (IHl a). congruence. lia.
+Qed.
+
+Lemma interp_prems_add V le (u : premises) :
+  interp_prems V (add le u) = Z.max (interp_expr V le) (interp_prems V u).
+Proof.
+  rewrite 2!interp_prems_elements.
+  erewrite fold_right_interp. 2:apply equivlistA_add.
+  rewrite fold_right_comm.
+  { apply map_nil, elements_not_empty. }
+  f_equal. eapply fold_right_equivlist_all.
+  have he := to_nonempty_list_spec u.
+  destruct to_nonempty_list. rewrite -he //=.
+Qed.
+
+Lemma interp_prems_eq (P : premises -> Z -> Prop) V :
+  (forall le, P (singleton le) (interp_expr V le)) ->
+  (forall le u k, P u k -> ~ LevelExprSet.In le u -> P (add le u) (Z.max (interp_expr V le) k)) ->
+  forall u, P u (interp_prems V u).
+Proof.
+  intros hs hadd.
+  eapply premises_elim.
+  - intros le. rewrite interp_prems_singleton. apply hs.
+  - intros le prems ih hnin.
+    rewrite interp_prems_add. now apply hadd.
+Qed.
+
+Lemma add_prems_singleton n cl : add_prems n (singleton cl) = singleton (add_expr n cl).
+Proof.
+  apply eq_univ_equal => [] [l k].
+  rewrite In_add_prems LevelExprSet.singleton_spec.
+  firstorder.
+  - destruct x; noconf H0.
+    eapply LevelExprSet.singleton_spec in H.
+    now red in H; noconf H.
+  - destruct cl. exists (t, z). split => //.
+    red in H; noconf H. now apply LevelExprSet.singleton_spec.
+Qed.
+
+Lemma interp_add_prems V n e : interp_prems V (add_prems n e) = n + interp_prems V e.
+Proof.
+  revert e.
+  refine (interp_prems_eq (fun u z => interp_prems V (add_prems n u) = n + z) _ _ _).
+  - intros le.
+    rewrite add_prems_singleton interp_prems_singleton //=.
+    destruct le; cbn. lia.
+  - intros le u k heq hnin.
+    rewrite add_prems_add.
+    rewrite interp_prems_add heq interp_add_expr. lia.
+Qed.
+
+Lemma in_pred_closure_entails cls cl :
+  in_pred_closure cls cl ->
+  (forall V, clauses_sem V cls -> clause_sem V cl).
+Proof.
+  induction 1.
+  - intros V. rewrite /clauses_sem. intros ha.
+    apply ha in H.
+    move: H; rewrite /clause_sem.
+    destruct cl as [prems concl].
+    cbn. rewrite interp_add_prems.
+    destruct concl as [concl conclk].
+    rewrite /add_expr; cbn. lia.
+  - intros V clsm. cbn.
+    rewrite interp_prems_singleton.
+    cbn. lia.
+Qed.
+
+Lemma interp_prems_in {V le} {u : premises} : LevelExprSet.In le u -> interp_prems V u >= interp_expr V le.
+Proof.
+  revert u.
+  refine (interp_prems_eq (fun u z => LevelExprSet.In le u -> z >= interp_expr V le) V _ _).
+  - intros le' u'.
+    apply LevelExprSet.singleton_spec in u'. red in u'; subst. lia.
+  - move=> le' u z hz hnin /LevelExprSet.add_spec [->|hin]. lia.
+    specialize (hz hin). lia.
+Qed.
+
+Lemma clauses_sem_subset {u u' : premises} : u ⊂_leset u' ->
+  forall V, interp_prems V u' >= interp_prems V u.
+Proof.
+  intros hsub V.
+  revert u u' hsub.
+  refine (interp_prems_eq (fun u z => forall u' : premises, u ⊂_leset u' -> interp_prems V u' >= z) V _ _).
+  - intros le u' hsing.
+    specialize (hsing le). forward hsing by now apply LevelExprSet.singleton_spec.
+    now apply interp_prems_in.
+  - intros le u k ih hin u' sub.
+    have hle := sub le.
+    specialize (ih u').
+    forward ih. intros x hin'. apply sub. now apply LevelExprSet.add_spec; right.
+    forward hle by now apply LevelExprSet.add_spec; left.
+    have hi := interp_prems_in (V := V) hle. lia.
+Qed.
+
+#[refine] Instance ge_refl : Reflexive Z.ge := _.
+Proof. red. lia. Qed.
+
+#[refine] Instance ge_trans : Transitive Z.ge := _.
+Proof. red. lia. Qed.
+
+Lemma clauses_sem_entails {cls cl} :
+  entails cls cl ->
+  (forall V, clauses_sem V cls -> clause_sem V cl).
+Proof.
+  induction 1.
+  - intros v clls. red.
+    destruct concl0 as [concl k].
+    have hge := interp_prems_ge v prems _ H.
+    by lia.
+  - move=> V Hcls.
+    move: {IHentails} (IHentails _ Hcls).
+    unfold clause_sem. unfold ge => hyp.
+    etransitivity; tea. rewrite interp_prems_add.
+    rewrite interp_prems_add in hyp.
+    eapply in_pred_closure_entails in H; tea.
+    move: H; rewrite /clause_sem. unfold ge.
+    have ssub := clauses_sem_subset H1 V. lia.
+Qed.
+
+Lemma clauses_sem_entails_all {cls prems concl} :
+  cls ⊢a prems → concl ->
+  (forall V, clauses_sem V cls -> interp_prems V prems >= interp_prems V concl).
+Proof.
+  intros ha V hcls.
+  red in ha.
+  move: ha.
+  revert concl.
+  refine (@interp_prems_eq (fun concl z => _ -> interp_prems V prems >= z) V _ _).
+  - move=> le //=. move/(_ le).
+    intros h; forward h by now apply LevelExprSet.singleton_spec.
+    now have ent := (clauses_sem_entails h _ hcls).
+  - intros le u k ih hnin.
+    intros hf.
+    forward ih. intros x hin; apply (hf x).
+    rewrite LevelExprSet.add_spec; now right.
+    specialize (hf le).
+    forward hf by now apply LevelExprSet.add_spec; left.
+    cbn in hf.
+    have ent := (clauses_sem_entails hf _ hcls). cbn in ent.
+    lia.
+Qed.
+
+Lemma infer_correct cls : infer_correctness cls.
+Proof.
+  unfold infer_correctness.
+  destruct infer_model as [m|] eqn:hi.
+  - (* Correct *) move: hi.
+    funelim (infer_model cls) => //.
+    intros [= <-].
+    set (obl := infer_model_obligation_1 cls). clearbody obl.
+    clear Heq Heqcall.
+    have mincl := model_incl vm.
+    destruct vm as [model ofV isupd clsconcl ism]; cbn in *.
+    set (V := clauses_levels cls) in *.
+    unfold correct_model.
+    have encl : enabled_clauses model cls.
+    { eapply enabled_clauses_ext. apply is_update_of_ext in isupd. exact isupd.
+      apply init_model_enabled. }
+    split => //.
+    unfold clauses_sem.
+    intros cl hin.
+    eapply valid_clause_model. now eapply encl in hin.
+    eapply Clauses.for_all_spec in ism; tc. now specialize (ism _ hin).
+  - intros [v clssem].
+    move: hi.
+    funelim (infer_model cls) => //. intros _.
+    red in islooping.
+    have sem := clauses_sem_entails_all islooping v0.
+    specialize (sem clssem).
+    rewrite interp_add_prems in sem. lia.
+Qed.
+
+Definition valid_entailment cls cl := forall V, clauses_sem V cls -> clause_sem V cl.
+
+Program Definition loop_check cls (cl : clause) : result (premises_model (clauses_levels cls) cl).1 LevelSet.empty cls (premises_model (clauses_levels cls) cl).2 :=
+  let V := clauses_levels cls in
+  loop (premises_model V cl).1 LevelSet.empty cls (premises_model V cl).2 (premises_model V cl).2 _.
+Next Obligation.
+  split => //.
+  - lsets.
+  - intros l. rewrite LevelSet.union_spec.
+    rewrite -/(LevelMap.In l (premises_model (clauses_levels cls) cl).2).
+    rewrite in_premises_model. intuition auto.
+  - apply is_update_of_empty.
+Qed.
+
+Definition premises_of_level_set (l : LevelSet.t) :=
+  LevelSet.fold (fun l acc => (l, 0) :: acc) l [].
+
+Definition extendV V (cl : clause) :=
+  let '(prems, concl) := cl in
+  (add_list (premises_of_level_set V) prems, concl).
+
+Lemma premises_model_map_min_premise {levels cls prems z} :
+  min_premise (premises_model_map (zero_model levels) cls) prems = Some z ->
+  (exists minp mink, LevelExprSet.In (minp, mink) prems /\
+    exists maxp, max_clause_premise_of minp cls = Some maxp /\
+    z = maxp - mink) \/
+  (exists minp mink, LevelExprSet.In (minp, mink) prems /\ z + mink <= 0)%Z.
+Proof.
+  set (m := premises_model_map _ _).
+  have [minple [[minp mink] [inminp mineq]]] := min_premise_spec m prems.
+  rewrite mineq. rewrite /min_atom_value.
+  destruct level_value eqn:hl => //. intros [= <-].
+  eapply level_value_MapsTo' in hl.
+  eapply premises_model_map_spec in hl as [[inpcls [hm _]]|[ninpcls h']]. left.
+  2:{ apply zero_model_spec in h' as [h' [= ->]]. }
+  exists minp, mink. split => //. noconf hm. rewrite -hm.
+  eexists; split => //.
+Qed.
+
+Lemma premises_model_map_min_premise_inv {levels cls} :
+  forall cl, Clauses.In cl cls ->
+  exists z, min_premise (premises_model_map (zero_model levels) cls) (premise cl) = Some z /\ (0 <= z)%Z.
+Proof.
+  set (m := premises_model_map _ _).
+  move=> cl hin.
+  have [minple [[minp mink] [inminp mineq]]] := min_premise_spec m (premise cl).
+  rewrite mineq. rewrite /min_atom_value.
+  destruct level_value eqn:hl => //.
+  - eexists. split; trea.
+    have ps := proj1 (premises_model_map_spec _ cls minp (Some z)) (level_value_MapsTo' hl).
+    destruct ps as [[minpsl [eq _]]|].
+    * symmetry in eq.
+      have sp := (max_clause_premise_of_spec _ _ _ _ hin inminp).
+      depelim sp. rewrite eq in H0. noconf H0. lia.
+    * destruct H. elim H.
+      eapply clauses_premises_levels_spec. exists cl. split => //.
+      eapply levelexprset_levels_spec. now exists mink.
+  - unfold level_value in hl.
+    destruct LevelMap.find eqn:hl'. subst o.
+    2:{ move/LevelMapFact.F.not_find_in_iff: hl'. elim.
+      rewrite premises_model_map_in. left.
+      eapply clauses_premises_levels_spec. exists cl. split => //.
+      eapply levelexprset_levels_spec. now exists mink. }
+    eapply LevelMap.find_2 in hl'.
+    move/premises_model_map_spec: hl' => [[]|[nin hm]] => //.
+    * now intros hnminp [_ hn].
+    * move: nin; elim.
+      eapply clauses_premises_levels_spec. exists cl. split => //.
+      eapply levelexprset_levels_spec. now exists mink.
+Qed.
+
+Lemma is_update_of_entails {cls V m m' hne hne'} : is_update_of cls V m m' ->
+  cls ⊢a of_level_map m hne → of_level_map m' hne'.
+Proof.
+  rewrite /is_update_of.
+  destruct LevelSet.is_empty.
+  - intros heq [].
+    rewrite !of_level_map_spec. rewrite -heq.
+    constructor. now apply of_level_map_spec.
+  - eapply strictly_updates_entails.
+Qed.
+
+Lemma is_update_of_non_empty {cls V m m'} : ~ LevelMap.Empty m ->
+  is_update_of cls V m m' ->
+  ~ LevelMap.Empty m'.
+Proof.
+  rewrite /is_update_of. destruct LevelSet.is_empty.
+  - now intros he <-.
+  - intros he su. now eapply strictly_updates_non_empty_map in su.
+Qed.
+
+Instance defined_map_proper : Proper (LevelMap.Equal ==> iff) defined_map.
+Proof.
+  intros x y eq; rewrite /defined_map.
+  now setoid_rewrite eq.
+Qed.
+
+Lemma is_update_of_defined_map {cls V m m'} : defined_map m ->
+  is_update_of cls V m m' ->
+  defined_map m'.
+Proof.
+  rewrite /is_update_of. destruct LevelSet.is_empty.
+  - now intros he <-.
+  - intros he su. now eapply strictly_updates_defined_map in su.
+Qed.
+
+Lemma inj_add_prems_sub {n u u'} : add_prems n u ⊂_leset add_prems n u' -> u ⊂_leset u'.
+Proof.
+  rewrite /add_prems.
+  intros hm [l k]. specialize (hm (l, k + n)).
+  rewrite !map_spec in hm.
+  intros hin.
+  forward hm. exists (l, k); split => //.
+  destruct hm as [[] [hin' eq]].
+  apply (@add_expr_inj n (l, k)) in eq. now noconf eq.
+Qed.
+
+Lemma premises_of_level_set_spec l k V : LevelSet.In l V /\ k = 0 <-> In (l, k) (premises_of_level_set V).
+Proof.
+  rewrite /premises_of_level_set.
+  eapply LevelSetProp.fold_rec.
+  - intros s' he. firstorder.
+  - intros x a s' s'' hin hnin hadd ih.
+    red in hadd. rewrite {}hadd.
+    cbn. firstorder. subst. now left. noconf H1. now left. now noconf H1.
+Qed.
+
+Lemma in_succ_add_premises {V u x k} : LevelExprSet.In (x, Z.of_nat (k + 1)) (add_list (premises_of_level_set V) u) -> LevelExprSet.In (x, Z.of_nat (k + 1)) u.
+Proof.
+  rewrite add_list_spec. intros [hn|hn] => //.
+  eapply premises_of_level_set_spec in hn as []. lia.
+Qed.
+
+(* Lemma inj_succ_prems {V u u'} : succ_prems u ⊂_leset add_list (premises_of_level_set V) u' -> succ_prems u ⊂_leset u'.
+Proof.
+  intros sub x. rewrite In_add_prems => [] [[l k] [hin ->]].
+  specialize (sub (l, Z.of_nat (k + 1))).
+  forward sub.
+  apply In_add_prems. exists (l, k). split => //.
+  now apply in_succ_add_premises in sub.
+Qed. *)
+
+Lemma succ_clauses_equiv cls prems concl :
+  succ_clauses cls ⊢ succ_prems prems → succ_expr concl ->
+  cls ⊢ prems → concl.
+Proof.
+  intros ha; depind ha.
+  - constructor.
+    move: H.
+    rewrite In_add_prems => [] [le [hin heq]].
+    move/add_expr_inj: heq. now intros ->.
+  - depelim H.
+    + destruct cl as [prems concl]. noconf H0.
+      eapply in_add_clauses in H as [[prems' concl'] [hin heq]].
+      noconf heq.
+      eapply (clause_cut _ (add_prems n prems') (add_expr n concl')). 2:eapply IHha.
+      2:{ f_equal. rewrite !add_expr_add_expr. now rewrite add_prems_add add_expr_add_expr Z.add_comm. }
+      exact: (incls cls (prems', concl') n hin).
+      rewrite add_prems_add_prems in H1. rewrite Z.add_comm in H1.
+      rewrite -(add_prems_add_prems 1 n prems') in H1.
+      now move/inj_add_prems_sub: H1.
+    + specialize (H0 (x, k + 1)). forward H0. now apply LevelExprSet.singleton_spec.
+      eapply In_add_prems in H0 as [[l' k'] [hin heq]]. noconf heq.
+      have eq: k' = k by lia. subst k'. clear H.
+      eapply clause_cut. 2:eapply IHha. eapply (predcl _ x (k - 1)).
+      2:{ intros x'. move/LevelExprSet.singleton_spec => ->. now have -> : k - 1 + 1 = k by lia. }
+      f_equal. rewrite add_prems_add. f_equal.
+      rewrite /succ_expr //=. lia_f_equal.
+Qed.
+
+Lemma entails_weak_list {cls prem concl concl'} :
+  cls ⊢ prem → concl ->
+  cls ⊢ add_list concl' prem → concl.
+Proof.
+  intros hcl.
+  induction concl' in prem, hcl |- *.
+  - exact hcl.
+  - cbn. eapply IHconcl'. now eapply entails_weak.
+Qed.
+
+Lemma entails_all_weak_list {cls prem concl concl'} :
+  entails_all cls prem concl ->
+  entails_all cls (add_list concl' prem) concl.
+Proof.
+  intros hcl x hin.
+  specialize (hcl _ hin). cbn in hcl.
+  now eapply entails_weak_list.
+Qed.
+
+Lemma premises_of_level_set_empty : premises_of_level_set LevelSet.empty = [].
+Proof.
+  now rewrite /premises_of_level_set LevelSetProp.fold_empty.
+Qed.
+
+(* Lemma succ_clauses_equiv_weak cls prems concl :
+  succ_clauses cls ⊢ succ_prems prems → succ_expr concl ->
+  cls ⊢ prems → concl.
+Proof.
+  move/(entails_weak_list (concl' := [])) => he.
+  eapply (succ_clauses_equiv _ LevelSet.empty).
+  cbn. now rewrite premises_of_level_set_empty.
+Qed. *)
+
+Lemma entails_all_succ_clauses cls prems concl :
+  succ_clauses cls ⊢a succ_prems prems → succ_prems concl ->
+  cls ⊢a prems → concl.
+Proof.
+  intros ha l hin. specialize (ha (succ_expr l)). forward ha.
+  eapply In_add_prems. exists l. split => //. cbn in ha.
+  now eapply succ_clauses_equiv in ha.
+Qed.
+
+Definition entails_equiv cls u u' :=
+  cls ⊢a u → u' /\ cls ⊢a u' → u.
+
+Notation "cls '⊢a' u ↔ u'" := (entails_equiv cls u u') (at level 90).
+
+Lemma max_premise_of_spec_aux s l k :
+  max_premise_of l s = k ->
+  (forall k', LevelExprSet.In (l, k') s -> (Some k' ≤ k)) /\
+  ((exists k', LevelExprSet.In (l, k') s /\ k = Some k') \/
+    ((~ exists k', LevelExprSet.In (l, k') s) /\ k = None)).
+Proof.
+  unfold max_premise_of.
+  revert k.
+  eapply LevelExprSetProp.fold_rec.
+  - intros s' he k <-. cbn. split => //.
+    * now move=> k' /he.
+    * right; split => //. now move=> [] k' /he.
+  - intros [l' k'] a s' s'' hin hnin hadd ih k.
+    specialize (ih _ eq_refl) as [hle hex].
+    intros hmax.
+    split. move=> k'0 /hadd => [] [].
+    { move=> [=] eq eq'. subst l' k'. rewrite eqb_refl in hmax.
+      destruct a; cbn in hmax; subst; constructor; lia. }
+    { move/hle. move: hmax. destruct (eqb_spec l l'); subst.
+      intros <-. intros h; depelim h; cbn. constructor; lia.
+      intros -> h; depelim h; constructor; lia. }
+    destruct hex as [[k'' [hin' heq]]|nex]. subst a.
+    { left. destruct (eqb_spec l l'). subst. exists (Z.max k' k''); split; trea.
+      2:{ subst k. eexists; split => //. apply hadd. now right. }
+      eapply hadd.
+      destruct (Z.max_spec k' k'') as [[hlt ->]|[hle' ->]] => //. now right. now left. }
+    destruct nex as [nex ->].
+    destruct (eqb_spec l l'). subst. left. exists k'. split => //. apply hadd; now left.
+    subst k. right. split => //.
+    intros [k'' hin']. apply hadd in hin' as []. noconf H0. congruence.
+    apply nex. now exists k''.
+Qed.
+
+Lemma max_premise_of_prems_max {l prems k} :
+  max_premise_of l prems = Some k -> LevelExprSet.In (l, k) prems.
+Proof.
+  destruct max_premise_of eqn:maxp => //. intros [= ->].
+  apply max_premise_of_spec_aux in maxp as [hle hex].
+  destruct hex as [[k' [hin [= ->]]]|hne] => //.
+  destruct hne; congruence.
+Qed.
+
+Lemma max_premise_of_singleton l k : max_premise_of l (singleton (l, k)) = Some k.
+Proof.
+  remember (max_premise_of l (singleton (l, k))) as mp. symmetry in Heqmp.
+  apply max_premise_of_spec_aux in Heqmp as [hle hex].
+  destruct hex as [[k' [hin heq]]|hne] => //.
+  eapply LevelExprSet.singleton_spec in hin. now noconf hin.
+  destruct hne as [nein ->]. elim nein.
+  exists k. now eapply LevelExprSet.singleton_spec.
+Qed.
+
+Lemma max_premise_of_spec2 l k (u : premises) : LevelExprSet.In (l, k) u ->
+  exists k', LevelExprSet.In (l, k') u /\ max_premise_of l u = Some k'.
+Proof.
+  remember (max_premise_of l u) as mp. symmetry in Heqmp.
+  apply max_premise_of_spec_aux in Heqmp as [hle hex].
+  intros hin. destruct hex. firstorder.
+  destruct H as [nein ->]. elim nein. now exists k.
+Qed.
+
+Lemma max_premise_of_spec_in l (u : premises) : LevelSet.In l (levels u) ->
+  exists k, max_premise_of l u = Some k /\ LevelExprSet.In (l, k) u.
+Proof.
+  intros hexi.
+  remember (max_premise_of l u) as mp. symmetry in Heqmp.
+  apply max_premise_of_spec_aux in Heqmp as [hle hex].
+  destruct hex. destruct H as [l' [hin heq]]. subst mp.
+  - eexists; split => //.
+  - destruct H as [nein ->]. elim nein.
+    now eapply levelexprset_levels_spec in hexi.
+Qed.
+
+(* Lemma of_level_map_premises_model_map cls cl V ne :
+  (forall l, LevelSet.In l (clause_levels cl) -> LevelSet.In l V) ->
+  cls ⊢a add_list (premises_of_level_set V) (premise cl) → of_level_map (premises_model_map (zero_model V) (Clauses.singleton cl)) ne.
+Proof.
+  intros hin [l k].
+  rewrite of_level_map_spec. move/premises_model_map_spec; cbn.
+  rewrite max_opt_of_l.
+  cbn; rewrite LevelSet.union_spec. firstorder try lsets.
+  cbn in H1.
+  - rewrite Z.max_comm.
+    destruct (Z.max_spec 0 (max_premise_of l (premise cl))) as [[hle ->]|[hge ->]].
+    * constructor. rewrite add_list_spec; right.
+      now eapply max_premise_of_spec_in.
+    * constructor. rewrite add_list_spec. left.
+      apply premises_of_level_set_spec. split => //.
+      apply hin. apply clause_levels_spec. now left.
+  - eapply zero_model_spec in H1 as [hin' [= ->]].
+Qed. *)
+
+(* Lemma max_premise_of_pos l prems : max_premise_of l prems >= 0.
+Proof.
+  have hs := max_premise_of_spec_aux prems l.
+  destruct max_premise_of. lia. lia.
+  specialize (hs _ eq_refl) as [_ [[k' []]|[_ hne]]]; lia.
+Qed.
+ *)
+
+Lemma of_level_map_premises_model_map cls cl V ne :
+  cls ⊢a premise cl → of_level_map (premises_model_map (zero_model V) (Clauses.singleton cl)) ne.
+Proof.
+  intros [l k].
+  rewrite of_level_map_spec. move/premises_model_map_spec; cbn.
+  intros [[hin' [[= heq] _]]|[hnin hm]].
+  2:{ now apply zero_model_spec in hm as []. }
+  move: hin'; cbn; rewrite LevelSet.union_spec. intros []; [|lsets].
+  eapply max_premise_of_spec_in in H as [maxp' [eq hin']].
+  rewrite eq in heq; noconf heq.
+  now constructor.
+Qed.
+
+Lemma entails_all_satisfies {cls prems m hne l k} :
+  cls ⊢a prems → of_level_map m hne ->
+  infers_atom m l k ->
+  cls ⊢ prems → (l, k).
+Proof.
+  intros hl hi.
+  eapply entails_all_one; tea. now apply infers_atom_of_level_map.
+Qed.
+
+Lemma premises_model_map_ne V cls :
+  ~ LevelMap.Empty V ->
+  ~ LevelMap.Empty (premises_model_map V cls).
+Proof.
+  intros ne he. apply ne.
+  have ne' := premises_model_map_in V cls.
+  intros l k hin.
+  specialize (ne' l). destruct ne'. forward H0. right. now exists k.
+  destruct H0 as [k' hin'].
+  now move/he: hin'.
+Qed.
+
+Lemma clauses_ne_exist cls : ~ Clauses.Empty cls -> exists cl, Clauses.In cl cls.
+Proof.
+  intros ne.
+  destruct (Clauses.choose cls) eqn:hc.
+  - exists e. now apply Clauses.choose_spec1 in hc.
+  - now apply Clauses.choose_spec2 in hc.
+Qed.
+
+Lemma premises_model_map_defined V cls :
+  ~ Clauses.Empty cls ->
+  defined_map (premises_model_map V cls).
+Proof.
+  move/clauses_ne_exist => [cl hin].
+  destruct cl as [prems concl].
+  pose proof (to_nonempty_list_spec' prems).
+  set (l := (to_nonempty_list prems).1) in *.
+  have hs := max_clause_premise_of_spec l l.2 cls (prems, concl) hin.
+  forward hs. cbn. eapply LevelExprSet.elements_spec1; rewrite -H.
+  constructor. destruct l; reflexivity. depelim hs.
+  exists l, y. apply premises_model_map_spec. left.
+  split => //.
+  eapply clauses_premises_levels_spec. eexists; split; tea => //.
+  rewrite //= levelexprset_levels_spec. exists l.2.
+  setoid_rewrite <- LevelExprSet.elements_spec1. rewrite -H //=.
+  constructor. destruct l; reflexivity.
+Qed.
+
+Variant check_result {cls} :=
+  | IsLooping (v : premises) (islooping : loop_on_univ cls v)
+  | Invalid
+  | Valid.
+Arguments check_result : clear implicits.
+
+Equations check_atom_value (z : option Z) (l : option Z) : bool :=
+  | Some _, None => false
+  | Some z, Some v => z <=? v
+  | None, _ => true.
+
+Lemma check_atom_value_spec z l : reflectProp (z ≤ l) (check_atom_value z l).
+Proof.
+  funelim (check_atom_value z l).
+  - destruct (Z.leb_spec z v); constructor.
+    * now constructor.
+    * intros h; depelim h. lia.
+  - constructor. intros h; depelim h.
+  - constructor. constructor.
+Qed.
+
+Lemma valid_model_find {V W cl cls} :
+  forall v : valid_model (clause_levels cl ∪ V) W (premises_model_map (zero_model (clause_levels cl ∪ V)) (Clauses.singleton cl)) cls,
+  ~ LevelMap.find (concl cl).1 (model_model v) = None.
+Proof.
+  intros v hfind.
+  destruct cl as [prems [concl k]]; cbn in *.
+  have vmupd := model_of_V v.
+  set (pm := premises_model_map _ _) in *.
+  move/LevelMapFact.F.not_find_in_iff: hfind; apply.
+  apply vmupd. rewrite LevelSet.union_spec; left.
+  rewrite clause_levels_spec. now right.
+Qed.
+
+Equations check (cls : clauses) (cl : clause) : check_result cls :=
+  check cls cl with loop_check cls cl :=
+    | Loop v isl => IsLooping v isl
+    | Model W v _ with inspect (LevelMap.find (concl cl).1 v.(model_model)) := {
+      | exist (Some val) he with check_atom_value (Some (concl cl).2) val :=
+        { | true => Valid
+          | false => Invalid }
+      | exist None he with valid_model_find v he := {}
+    }.
+
+Definition check_clauses (cls : clauses) (cls' : clauses) : bool :=
+  let check_one cl :=
+    match check cls cl with
+    | IsLooping v isl => false
+    | Valid => true
+    | Invalid => false
+    end
+  in
+  Clauses.for_all check_one cls'.
+
+(* If a clause checks, then it should be valid in any extension of the model *)
+Lemma check_entails {cls cl} :
+  check cls cl = Valid -> valid_entailment cls cl.
+Proof.
+  destruct cl as [prems [concl k]].
+  funelim (check cls _) => // _.
+  set (V := clause_levels _ ∪ clauses_levels cls) in *.
+  clear Heqcall H. cbn [concl fst snd] in *. clear Heq0.
+  unfold valid_entailment, valid_clause, level_value_above.
+  move/check_atom_value_spec: Heq; intros h; depelim h. rename H into hgt.
+  intros valuation ext.
+  have vmupd := model_updates v.
+  have vmok := model_ok v.
+  set (pm := premises_model_map _ _) in *.
+  have nepm : defined_map pm.
+  { apply premises_model_map_defined.
+    set (cl := (prems, _)) in *.
+    move/(_ cl). rewrite Clauses.singleton_spec. congruence. }
+  have nev : defined_map (model_model v).
+    by apply (is_update_of_defined_map nepm vmupd).
+  move/(is_update_of_entails (hne := nepm) (hne' := nev)): vmupd => ent.
+  set (cl := (prems, (concl0, k))) in V.
+  have of_lset := of_level_map_premises_model_map cls cl V nepm.
+  have tr := entails_all_trans of_lset ent.
+  eapply (entails_all_satisfies (l := concl0) (k := k)) in tr.
+  2:{ red. rewrite /level_value he. now constructor. }
+  eapply clauses_sem_entails in tr ; tea.
+Qed.
+
+Definition invalid_entailment cls cl :=
+  forall V, clauses_sem V cls -> clause_sem V cl -> False.
+
+Definition infers_univ (m : model) (u : premises) :=
+  exists z, min_premise m u = Some z /\ (0 <= z)%Z.
+
+Definition infers_expr (m : model) (le : LevelExpr.t) :=
+  let '(l, k) := le in infers_atom m l k.
+
+Lemma valid_clause_elim {m prems concl k} : valid_clause m (prems, (concl, k)) ->
+  forall z, min_premise m prems = Some z ->
+  Some (z + k) ≤ level_value m concl.
+Proof.
+  rewrite /valid_clause => hcl z eqmin.
+  rewrite eqmin in hcl. cbn in *.
+  move: hcl. rewrite /level_value_above. destruct level_value eqn:hl => //.
+  move/Z.leb_le. constructor. lia.
+Qed.
+
+Lemma valid_clause_intro {m prems concl k} :
+  (forall z,
+    min_premise m prems = Some z ->
+    Some (z + k) ≤ level_value m concl) ->
+  valid_clause m (prems, (concl, k)).
+Proof.
+  rewrite /valid_clause //=.
+  destruct min_premise => //.
+  intros hz.
+  specialize (hz _ eq_refl). depelim hz.
+  rewrite /level_value_above H0.
+  apply Z.leb_le. lia.
+Qed.
+
+Lemma infers_expr_min_atom_value m le : infers_expr m le -> exists k, min_atom_value m le = Some k /\ (0 <= k)%Z.
+Proof.
+  destruct le as [l k]; rewrite /infers_expr //=.
+  rewrite /infers_atom. destruct level_value => // hle; depelim hle.
+  eexists; split; trea. lia.
+Qed.
+
+Lemma min_premise_add_infers m prems le lev :
+  level_value m le.1 = Some lev ->
+  forall z, min_premise m prems = Some z ->
+  exists z', min_premise m (add le prems) = Some z' /\
+    ((z' = lev - le.2 /\ z' <= z) \/ z' = z).
+Proof.
+  intros hlev z hmin.
+  have [hle [min' [hin hm]]] := min_premise_spec m (add le prems).
+  have [hle' [min'' [hin' hm']]] := min_premise_spec m prems.
+  move/LevelExprSet.add_spec: hin => [heq|hin].
+  - noconf heq. destruct le as [le k].
+    rewrite /min_atom_value hlev in hm.
+    eexists; split => //; trea. left.
+    specialize (hle min''). forward hle.
+    { rewrite LevelExprSet.add_spec. now right. }
+    rewrite hm -hm' hmin in hle. now depelim hle.
+  - exists z. split => //. 2:right; reflexivity. rewrite hm -hmin hm'.
+    move: (hle' _ hin). rewrite hmin. intros h; depelim h.
+    rewrite H0 in hm.
+    specialize (hle min''). forward hle. eapply LevelExprSet.add_spec. now right.
+    rewrite hm in hle. rewrite -hm' hmin in hle. depelim hle.
+    rewrite H0 -hm' hmin. f_equal. lia.
+Qed.
+
+Lemma fold_left_map {A B C} (f : B -> A -> A) (g : C -> B) l acc :
+  fold_left (fun acc l => f (g l) acc) l acc =
+  fold_left (fun acc l => f l acc) (List.map g l) acc.
+Proof.
+  induction l in acc |- *; cbn; auto.
+Qed.
+
+Lemma fold_left_max_acc {n l} : (forall x, In x l -> x = n) -> n = fold_left (option_map2 Z.min) l n.
+Proof.
+  induction l in n |- *.
+  - now cbn.
+  - cbn. intros he. transitivity (option_map2 Z.min n a). 2:apply IHl.
+    specialize (he a). forward he. now left. subst. destruct n => //= //. lia_f_equal.
+    intros. have h := (he x). forward h by now right.
+    have h' := (he a). forward h' by now left. subst.
+    destruct n => //=; lia_f_equal.
+Qed.
+
+Lemma option_map2_comm x y : option_map2 Z.min x y = option_map2 Z.min y x.
+Proof.
+  destruct x, y; cbn; lia_f_equal.
+Qed.
+
+Lemma option_map2_assoc x y z :
+  option_map2 Z.min x (option_map2 Z.min y z) =
+  option_map2 Z.min (option_map2 Z.min x y) z.
+Proof.
+  destruct x, y, z; cbn; lia_f_equal.
+Qed.
+
+Local Notation fn := (fold_left (option_map2 Z.min)).
+
+Lemma fold_left_impl n l :
+  (forall x, In x (n :: l) -> fn l n ≤ x) /\
+  (exists x, In x (n :: l) /\ fn l n = x).
+Proof.
+  induction l in n |- *.
+  - cbn. split; intros.
+    destruct H => //. subst. reflexivity.
+    exists n. split => //. now left.
+  - cbn. split; intros.
+    { destruct (IHl n) as [hle [min [hin heq]]].
+    rewrite fold_left_comm.
+    { now intros; rewrite -option_map2_assoc (option_map2_comm x0 y) option_map2_assoc. }
+    repeat destruct H; subst.
+    * specialize (hle n). forward hle. now left.
+      transitivity (fn l n); auto. eapply Zmin_opt_left.
+    * eapply Zmin_opt_right.
+    * transitivity (fn l n); auto. apply Zmin_opt_left.
+      apply hle. now right. }
+    * specialize (IHl (option_map2 Z.min n a)).
+      destruct IHl as [hle [min [hin heq]]]. subst min. eexists. split; trea.
+      destruct hin.
+      rewrite -H.
+      destruct n, a; cbn; firstorder.
+      destruct (Z.min_spec z z0) as [[? heq]|[? heq]].
+      rewrite -{1}heq. now left. right; left. f_equal. lia.
+      now right.
+Qed.
+
+Lemma fold_left_impl_eq n n' l l' :
+  (forall x, In x (n :: l) <-> In x (n' :: l' )) ->
+  fn l n = fn l' n'.
+Proof.
+  intros heq.
+  destruct (fold_left_impl n l) as [hle [minl [hin heq']]].
+  destruct (fold_left_impl n' l') as [hle' [minl' [hin' heq'']]].
+  rewrite heq' heq''.
+  specialize (hle minl'). forward hle. now apply heq.
+  specialize (hle' minl). forward hle'. now apply heq.
+  rewrite heq'' in hle'. rewrite heq' in hle. depelim hle'. depelim hle. f_equal; lia.
+  now depelim hle.
+Qed.
+
+Lemma fold_left_comm_f {A} (f : A -> A -> A) n l :
+  (forall x y, f x y = f y x) ->
+  fold_left f l n = fold_left (flip f) l n.
+Proof.
+  induction l in n |- *; cbn; auto.
+  intros hf. rewrite IHl //.
+  unfold flip. now rewrite hf.
+Qed.
+
+Lemma min_premise_add {m le prems} : min_premise m (add le prems) =
+  option_map2 Z.min (min_atom_value m le) (min_premise m prems).
+Proof.
+  rewrite {1}/min_premise.
+  have hs' := to_nonempty_list_spec (add le prems).
+  destruct to_nonempty_list.
+  have eqf : (fold_left (fun (min : option Z) (atom : LevelExpr.t) => option_map2 Z.min (min_atom_value m atom) min) l (min_atom_value m p)) =
+    (option_map2 Z.min (min_atom_value m le) (min_premise m prems)).
+  2:{ now rewrite eqf. }
+  rewrite -(to_nonempty_list_spec' (add le prems)) in hs'. noconf hs'.
+  rewrite fold_left_map. rewrite fold_left_comm_f. intros [] []; cbn; auto. lia_f_equal. unfold flip.
+  have l := fold_left_impl_eq (min_atom_value m (to_nonempty_list (add le prems)).1) (min_atom_value m le)
+    (List.map (min_atom_value m) (to_nonempty_list (add le prems)).2) (List.map (min_atom_value m) (LevelExprSet.elements prems)).
+  rewrite l.
+  intros x.
+  { rewrite -!map_cons to_nonempty_list_spec' !in_map_iff.
+    split.
+    - move=> [] lk [] <-.
+      rewrite -InA_In_eq.
+      move/LevelExprSet.elements_spec1.
+      rewrite LevelExprSet.add_spec.
+      intros [->|inp].
+      * exists le. split => //. now left.
+      * exists lk. split => //. right. now apply InA_In_eq, LevelExprSet.elements_spec1.
+    - intros [x' [<- hin]].
+      exists x'. split => //. rewrite -InA_In_eq.
+      eapply LevelExprSet.elements_spec1. rewrite LevelExprSet.add_spec.
+      apply InA_In_eq in hin. depelim hin. now left.
+      eapply LevelExprSet.elements_spec1 in hin. now right. }
+  rewrite option_map2_comm.
+  rewrite /min_premise.
+  destruct (to_nonempty_list prems) eqn:he.
+  rewrite fold_left_map.
+  rewrite (fold_left_comm_f _ _ (List.map _ l0)). intros. apply option_map2_comm.
+  rewrite -(fold_left_comm (option_map2 Z.min)).
+  { intros. now rewrite -option_map2_assoc (option_map2_comm x y) option_map2_assoc. }
+  rewrite -(to_nonempty_list_spec' prems) he; cbn.
+  now rewrite option_map2_comm.
+Qed.
+
+Lemma min_premise_elim m (P : premises -> option Z -> Prop):
+  (forall le, P (singleton le) (min_atom_value m le)) ->
+  (forall prems acc le, P prems acc -> ~ LevelExprSet.In le prems -> P (add le prems) (option_map2 Z.min (min_atom_value m le) acc)) ->
+  forall prems, P prems (min_premise m prems).
+Proof.
+  intros hs hadd.
+  eapply premises_elim.
+  - intros le. rewrite /min_premise.
+    rewrite singleton_to_nonempty_list. cbn. apply hs.
+  - intros le prems hp. now rewrite min_premise_add.
+Qed.
+
+Lemma min_premise_add_down {m} {prems : premises} {l k} :
+  LevelExprSet.In (l, k + 1) prems ->
+  forall z, min_premise m prems = Some z ->
+       min_premise m (add (l, k) prems) = Some z.
+Proof.
+  intros ine z hmin.
+  have [hle [min' [hin hm]]] := min_premise_spec m (add (l, k) prems).
+  have [hle' [min'' [hin' hm']]] := min_premise_spec m prems.
+  move/LevelExprSet.add_spec: hin => [heq|hin].
+  - noconf heq.
+    specialize (hle (l, k + 1)).
+    forward hle. eapply LevelExprSet.add_spec. now right.
+    rewrite hm in hle.
+    depelim hle. destruct level_value eqn:hl. noconf H0; noconf H1. lia. congruence.
+    destruct level_value eqn:hl' => //.
+    specialize (hle' _ ine). rewrite hmin in hle'; depelim hle'.
+    now rewrite hl' in H1.
+  - rewrite hm. specialize (hle' min' hin). rewrite hmin in hle'.
+    depelim hle'. rewrite H0. f_equal. rewrite H0 in hm.
+    specialize (hle min''). forward hle. eapply LevelExprSet.add_spec. now right.
+    rewrite hm in hle. rewrite -hm' hmin in hle. depelim hle. lia.
+Qed.
+
+
+Lemma min_premise_singleton m u : min_premise m (singleton u) = min_atom_value m u.
+Proof.
+  now rewrite /min_premise singleton_to_nonempty_list; cbn.
+Qed.
+
+Lemma min_atom_value_add m e x n :
+  min_atom_value m e = Some x ->
+  min_atom_value m (add_expr n e) = Some (x - n)%Z.
+Proof.
+  rewrite /min_atom_value. destruct e. cbn.
+  destruct level_value => //. intros [= <-].
+  f_equal. lia.
+Qed.
+
+
+Lemma min_atom_value_add_inv m e x n :
+  min_atom_value m (add_expr n e) = Some x ->
+  min_atom_value m e = Some (x + n)%Z.
+Proof.
+  rewrite /min_atom_value. destruct e. cbn.
+  destruct level_value => //. intros [= <-].
+  f_equal. lia.
+Qed.
+
+Lemma min_premise_add_prems {m n prems z} : min_premise m prems = Some z -> min_premise m (add_prems n prems) = Some (z - n)%Z.
+Proof.
+  revert z.
+  eapply min_premise_elim.
+  - intros le hm.
+    destruct le as [concl k].
+    rewrite add_prems_singleton min_premise_singleton.
+    apply min_atom_value_add.
+  - intros prems' acc le ih nle z hm.
+    destruct acc; cbn in hm. 2:{ destruct (min_atom_value m le); cbn in hm; congruence. }
+    specialize (ih _ eq_refl).
+    rewrite add_prems_add min_premise_add.
+    destruct (min_atom_value m le) eqn:hm'; cbn in hm => //. noconf hm.
+    apply (min_atom_value_add _ _ _ n) in hm'.
+    rewrite ih hm'. cbn. f_equal. lia.
+Qed.
+
+Lemma min_premise_add_prems_inv {m n prems z} : min_premise m (add_prems n prems) = Some z ->
+  min_premise m prems = Some (z + n)%Z.
+Proof.
+  revert z.
+  pattern prems.
+  set (P := (fun n0 hm =>
+  forall z : Z,
+    min_premise m (add_prems n n0) = Some z -> hm = Some (z + n)%Z)).
+  apply (@min_premise_elim _ P); subst P; cbn.
+  - intros le z hm.
+    destruct le as [concl k].
+    rewrite add_prems_singleton min_premise_singleton in hm.
+    now apply min_atom_value_add_inv.
+  - intros prems' acc le ih nle z.
+    rewrite add_prems_add min_premise_add.
+    destruct (min_premise m (add_prems n prems')) eqn:he => //=.
+    * destruct (min_atom_value m (add_expr n le)) eqn:ha => //=.
+      intros [= <-].
+      eapply min_atom_value_add_inv in ha. rewrite ha.
+      specialize (ih _ eq_refl). subst acc. cbn. lia_f_equal.
+    *  destruct (min_atom_value m (add_expr n le)) eqn:ha => //=.
+Qed.
+
+Lemma level_value_above_leq {m l k} :
+  Some k ≤ level_value m l ->
+  level_value_above m l k.
+Proof.
+  intros h; rewrite /level_value_above.
+  depelim h. rewrite H0. apply Z.leb_le. lia.
+Qed.
+
+Lemma valid_clause_shift m n cl :
+  valid_clause m cl -> valid_clause m (add_clause n cl).
+Proof.
+  destruct cl as [prems [concl k]].
+  move/valid_clause_elim => hv.
+  apply valid_clause_intro => z eqmin.
+  eapply min_premise_add_prems_inv in eqmin.
+  specialize (hv _ eqmin).
+  etransitivity; tea. constructor; lia.
+Qed.
+
+Lemma entails_model_valid cls cl : entails cls cl ->
+  forall m, is_model cls m -> valid_clause m cl.
+Proof.
+  induction 1.
+  - intros m ism.
+    destruct concl0 as [concl k].
+    apply valid_clause_intro => z hmin.
+    eapply min_premise_spec_aux in hmin as [hle [x [hin heq]]].
+    specialize (hle _ H). depelim hle.
+    destruct level_value eqn:hl => //. noconf H1.
+    constructor. lia.
+  - intros.
+    specialize (IHentails m H2).
+    depelim H.
+    * destruct cl as [premsc conclc].
+      noconf H0.
+      eapply Clauses.for_all_spec in H3.
+      eapply H3 in H. 2:tc.
+      destruct concl0 as [concl k].
+      eapply valid_clause_intro => z eqmin.
+      have mins := min_premise_subset m (add_prems n premsc) prems H2.
+      rewrite eqmin in mins; depelim mins.
+      destruct conclc as [conclc k'].
+      have vshift : valid_clause m (add_prems n premsc, add_expr n (conclc, k')).
+      { now eapply (valid_clause_shift _ n) in H. }
+      have hv := valid_clause_elim vshift _ H4.
+      depelim hv. rename y0 into vmconclc.
+      eapply (min_premise_add_infers _ _ (add_expr n (conclc, k'))) in eqmin as [minadd [eqminadd disj]]; tea.
+      move/valid_clause_elim: IHentails => //=.
+      move/(_ _ eqminadd).
+      destruct disj as [[eq le']| ->].
+      + move=> h. cbn in le'. cbn in eq. subst minadd.
+        depelim h. rewrite H8. constructor. lia.
+      + intros h; depelim h. rewrite H8; constructor; lia.
+    * destruct concl0 as [concl0 k'].
+      apply valid_clause_intro => z hmin.
+      have mins := min_premise_subset m _ _ H1.
+      rewrite min_premise_singleton in mins.
+      specialize (H1 (x, k+1)); forward H1 by now apply LevelExprSet.singleton_spec.
+      have hadd := min_premise_add_down H1 _ hmin.
+      exact: valid_clause_elim IHentails _ hadd.
+Qed.
+
+Lemma check_entails_looping {cls cl v isl} :
+  check cls cl = IsLooping v isl -> cls ⊢a v → succ_prems v.
+Proof.
+  funelim (check cls cl) => //.
+Qed.
+
+Lemma enabled_clause_ext {m m' cl} :
+  m ⩽ m' -> enabled_clause m cl -> enabled_clause m' cl.
+Proof.
+  intros hext; rewrite /enabled_clause.
+  destruct cl as [prems [concl k]]; cbn; move=> [z hm].
+  have pr := min_premise_pres prems hext.
+  rewrite hm in pr. depelim pr. now exists y.
+Qed.
+
+Lemma check_entails_false {cls cl} :
+  check cls cl = Invalid -> ~ entails cls cl.
+Proof.
+  funelim (check cls cl) => //.
+  set (V := clause_levels cl ∪ clauses_levels cls) in *.
+  destruct cl as [prems [concl k]].
+  rename val into conclval_v => _. clear H Heq0 Heqcall prf. cbn in he.
+  move: (check_atom_value_spec (Some k) conclval_v). rewrite Heq.
+  intros r; depelim r. rename H into nent. intros H.
+  have vmupd := model_updates v.
+  have vmok := model_ok v.
+  set (pm := premises_model_map _ _) in *.
+  set (cl := (prems, _)) in V.
+  have nepm : defined_map pm.
+  { apply premises_model_map_defined.
+    move/(_ cl). rewrite Clauses.singleton_spec /cl. congruence. }
+  have nev : defined_map (model_model v).
+    by apply (is_update_of_defined_map nepm vmupd).
+  move/(is_update_of_entails (hne := nepm) (hne' := nev)): vmupd => ent.
+  move/entails_model_valid/(_ _ vmok): H.
+  have [z minp] : enabled_clause (model_model v) cl.
+  { apply (@enabled_clause_ext pm).
+    exact: is_update_of_ext (model_updates v).
+    red; cbn.
+    have hcl : Clauses.In cl (Clauses.singleton cl).
+    { now eapply Clauses.singleton_spec. }
+    have hs:= @premises_model_map_min_premise_inv V _ _ hcl. firstorder. }
+  move/valid_clause_elim/(_ z minp).
+  cbn in minp.
+  rewrite /level_value he => h; depelim h. apply nent.
+  constructor.
+  have posz : 0 <= z.
+  { have hsu := model_updates v.
+    eapply is_update_of_ext in hsu.
+    have hs := min_premise_pres prems hsu.
+    rewrite minp in hs.
+    have hmin := @premises_model_map_min_premise_inv V (Clauses.singleton cl) cl.
+    forward hmin. now apply Clauses.singleton_spec.
+    destruct hmin as [minp' [hmineq hpos]].
+    rewrite hmineq in hs. depelim hs. lia. }
+  lia.
+Qed.
+
+Equations? infer_model_extension (V : LevelSet.t) (m : model) (cls cls' : clauses)
+  (prf : clauses_levels cls ⊂_lset V /\ clauses_levels cls' ⊂_lset V /\ only_model_of V m) : result V LevelSet.empty (Clauses.union cls cls') m :=
+  | V, m, cls, cls', prf := loop V LevelSet.empty (Clauses.union cls cls') m m _.
+Proof.
+  split.
+  - intros x. rewrite clauses_levels_spec.
+    move=> [] cl. rewrite Clauses.union_spec.
+    intros [[] incls]. apply H. apply clauses_levels_spec. exists cl. split => //.
+    apply H0. apply clauses_levels_spec. exists cl; split => //.
+  - exact H1.
+  - eapply is_update_of_empty.
+Qed.
+
+
+(* To infer an extension, we weaken a valid model for V to a model for [V ∪ clauses_levels cls] by
+   setting a minimal value for the new atoms in [clauses_levels cls \ V]
+   such that the new clauses [cls] do not hold vacuously.
+*)
+
+Equations add_max (l : Level.t) (k : option Z) (m : model) : model :=
+add_max l k m with level_value m l :=
+  { | Some k' with check_atom_value k (Some k') :=
+    { | true => m
+      | false => LevelMap.add l k m }
+  | None => LevelMap.add l k m }.
+
+Lemma nleq_optZ k k' : ~ k ≤ Some k' -> exists z, k = Some z /\ k' < z.
+Proof.
+  destruct k.
+  - exists z. split => //. eapply Znot_ge_lt => hl; apply H. constructor. lia.
+  - elim. constructor.
+Qed.
+
+Lemma add_max_spec l l' k k' (m : model) :
+  LevelMap.MapsTo l k (add_max l' k' m) <->
+  (l = l' /\ k = max_opt_of Z.max k' (level_value m l)) \/
+  (l <> l' /\ LevelMap.MapsTo l k m).
+Proof.
+  funelim (add_max l' k' m).
+  - rewrite LevelMapFact.F.add_mapsto_iff /Level.eq. firstorder; subst.
+    left. split => //. rewrite Heq. now rewrite max_opt_of_l.
+    left. firstorder. now rewrite Heq max_opt_of_l.
+  - clear Heqcall.
+    destruct (eq_dec l0 l).
+    * subst l0. rewrite Heq0.
+      move/check_atom_value_spec: Heq.
+      rewrite (maps_to_update (level_value_MapsTo' Heq0)).
+      firstorder; subst; try left; try split; auto; depelim Heq; cbn; lia_f_equal.
+    * firstorder.
+  - rewrite LevelMapFact.F.add_mapsto_iff /Level.eq.
+    have := check_atom_value_spec k (Some k'). rewrite {}Heq.
+    intros h; depelim h. apply nleq_optZ in H as [z [-> hlt]].
+    firstorder; subst.
+    * left; split => //. rewrite Heq0 //=. lia_f_equal.
+    * left; split => //. rewrite Heq0 //=. lia_f_equal.
+Qed.
+
+Definition min_model_clause cl m :=
+  LevelExprSet.fold (fun '(l, k) acc => add_max l (Some k) acc) (premise cl)
+    (add_max (concl cl) None m).
+
+Definition min_model_map (m : model) cls : model :=
+  Clauses.fold min_model_clause cls m.
+
+Lemma In_add_max l l' k acc :
+  LevelMap.In l (add_max l' k acc) <-> (l = l' \/ LevelMap.In l acc).
+Proof.
+  rewrite /LevelMap.In.
+  rw add_max_spec. firstorder subst.
+  eexists; left; eauto.
+  destruct (eq_dec l l'); subst; eexists; eauto.
+Qed.
+
+Definition is_max k' k l acc :=
+  match LevelMap.find l acc with
+  | Some k'' => k' = Nat.max k k''
+  | _ => k' = k
+  end.
+
+Lemma max_opt_of_spec {x y k'} : max_opt_of Z.max x y = k' ->
+  (x ≤ y /\ k' = y) \/ (y ≤ x /\ k' = x).
+Proof.
+  destruct x, y; cbn; firstorder subst.
+  - destruct (Z.max_spec z z0) as [[]|[]];
+    [left|right]; split; try constructor; lia_f_equal.
+  - right. split; constructor.
+  - left. split; constructor.
+  - left; split; constructor.
+Qed.
+
+Definition max_of_premises l kl n :=
+  (forall kl', LevelExprSet.In (l, kl') n -> Some kl' ≤ kl).
+
+Definition is_expr l (e : LevelExpr.t) :=
+  let '(concl, k) := e in concl = l.
+
+Definition max_of_clause l kl cl :=
+  max_of_premises l kl (premise cl).
+
+Definition max_of_map l kl m :=
+  (forall kl', LevelMap.MapsTo l kl' m -> kl' ≤ kl).
+
+Definition is_max_of_clause_and_map l cl m k :=
+  max_of_premises l k (premise cl) /\ max_of_map l k m.
+
+Definition is_in_premise l k (u : LevelExprSet.t) :=
+  (exists kl, LevelExprSet.In (l, kl) u /\ k = Some kl).
+
+Definition is_in_clause l k (cl : clause) :=
+  is_in_premise l k (premise cl) \/ (l = (clause_conclusion cl) /\ k = None).
+
+Definition is_max_of_clause_model l cl m k :=
+  is_max_of_clause_and_map l cl m k /\
+  (is_in_clause l k cl \/ LevelMap.MapsTo l k m).
+
+Definition is_higher l k m := exists k', LevelMap.MapsTo l k' m /\ k ≤ k'.
+
+Definition is_max_of_clause_map (map : model) l cl (m : model) : Prop :=
+  (forall k, LevelMap.MapsTo l k map -> is_max_of_clause_model l cl m k)
+  /\ (forall l k, LevelMap.MapsTo l k m \/ is_in_clause l k cl -> is_higher l k map).
+
+
+Lemma max_opt_of_le_l z z' : z ≤ max_opt_of Z.max z z'.
+Proof.
+  destruct z, z'; cbn; constructor; lia.
+Qed.
+
+Lemma max_opt_of_le_r z z' : z' ≤ max_opt_of Z.max z z'.
+Proof.
+  destruct z, z'; cbn; constructor; lia.
+Qed.
+
+Lemma is_higher_le l k l' k' m : is_higher l k m -> is_higher l k (add_max l' k' m).
+Proof.
+  rewrite /is_higher.
+  rw add_max_spec.
+  intros [k'0 [hm hle]].
+  destruct (eq_dec l l').
+  - subst. eexists. split; eauto. rewrite (level_value_MapsTo hm).
+    transitivity k'0 => //. apply max_opt_of_le_r.
+  - exists k'0. split; eauto.
+Qed.
+
+Lemma is_higher_add l k m : is_higher l k (add_max l k m).
+Proof.
+  rewrite /is_higher.
+  rw add_max_spec. eexists. split; eauto.
+  apply max_opt_of_le_l.
+Qed.
+
+Lemma is_higher_mon l k k' m : is_higher l k' m -> k ≤ k' -> is_higher l k m.
+Proof.
+  intros [? []] le. exists x. split => //. now transitivity k'.
+Qed.
+
+Lemma MapsTo_fold_add_max l n a :
+  let map := LevelExprSet.fold (fun '(l, k0) acc => add_max l (Some k0) acc) n a in
+  (forall k, LevelMap.MapsTo l k map ->
+  ((exists kl,
+    [/\ LevelExprSet.In (l, kl) n, k = Some kl,
+    (forall kl', LevelExprSet.In (l, kl') n -> kl' <= kl) &
+    (forall kl', LevelMap.MapsTo l kl' a -> kl' ≤ Some kl)]) \/
+    (LevelMap.MapsTo l k a /\ (forall kl', LevelExprSet.In (l, kl') n -> Some kl' ≤ k))))
+  /\ (forall l k, LevelMap.MapsTo l k a \/ is_in_premise l k n -> is_higher l k map) /\
+  a ⩽ map.
+   (* ~ LevelMap.In l map -> ~ (exists k, LevelExprSet.In (l, k) n) /\ ~ (LevelMap.In l a)). *)
+Proof.
+  eapply LevelExprSetProp.fold_rec.
+  - intros s' he. cbn.
+    rewrite /is_in_premise /is_higher.
+    setoid_rewrite (LevelExprSetProp.empty_is_empty_1 he).
+    intuition auto. right. split; eauto.
+    intros kl. now move/LevelExprSet.empty_spec.
+    exists k; split => //. reflexivity.
+    destruct H0 as [x [hin ->]]. now apply LevelExprSet.empty_spec in hin.
+    reflexivity.
+  - cbn; intros.
+    destruct x as [xl k']. split.
+    2:{ split.
+      { intros l0 hnin. destruct H2 as [hm [H2 _]]. specialize (H2 l0).
+      intros [ina|ins''].
+      { specialize (H2 hnin (or_introl ina)). eapply is_higher_le; tea. }
+      { destruct ins'' as [x [ins'' ->]].
+        apply H1 in ins'' as [[=]|ins'].
+        * subst. apply is_higher_add.
+        * apply is_higher_le, H2. right. eexists; eauto. } }
+      { destruct H2 as [_ [_ H2]].
+        intros l' hin. move/H2 => [k'0 [hm hle]].
+        rw add_max_spec. destruct (eq_dec l' xl).
+        - eexists; split. left; eauto. subst l'.
+          rewrite (level_value_MapsTo hm). transitivity (k'0) => //.
+          apply max_opt_of_le_r.
+        - eexists; split; eauto. } }
+    intros.
+    rewrite add_max_spec in H3; destruct H3 as [[<- hk]|[hdiff hm]].
+    * destruct H2 as [hin hnin]. symmetry in hk.
+      have [[leacc eqms]|[len eqms]] := max_opt_of_spec hk.
+      { depelim leacc. specialize (hin _ (level_value_MapsTo' H3)) as [[kl [inkl [= <-] les' lea]]|].
+        { left. exists y. split => //. apply H1; now right. congruence. intros.
+          apply H1 in H4 as [[=]|ins']. 2:now apply les'. subst kl'. lia. }
+        { destruct H4. right. split. now rewrite -H3 -eqms in H4. intros.
+          apply H1 in H6 as [[=]|ins']; subst; trea. rewrite H3; cbn; constructor; lia_f_equal.
+          rewrite H3; cbn; constructor. apply H5 in ins'. depelim ins'. lia. } }
+      { left. exists k'. split => //.
+        * apply H1. now left.
+        * move=> kl' /H1 [[=]|ins']. lia. depelim len. transitivity x; tea. specialize (hin _ (level_value_MapsTo' H3)) as
+         [[kl [inkl [= <-] les' lea]]|[]].
+          { now eapply les'. }
+          { specialize (H5 _ ins'). depelim H5. lia. }
+          { move: H2 hk. rewrite /level_value. destruct (find_spec l a0).
+            * intros ->. apply hin in H2 as [[kl []]|[hm hkl']] => //. apply hkl' in ins'. depelim ins'.
+            * intros _; cbn; intros <-.
+              destruct hnin as [hnin _].
+              specialize (hnin l (Some kl')); forward hnin. right.
+              red. exists kl'. split => //.
+              destruct hnin as [ka [hma hge]]. elim H2. now exists ka. }
+        * subst k. intros kl' mt. move: len. case: level_valueP => [k ma0 le|].
+          specialize (hin _ ma0) as [[kl []]|[hm hkl']] => //.
+          + subst k. eapply H5 in mt. now depelim le; depelim mt; constructor; lia.
+          + transitivity k => //. eapply LevelMapFact.F.MapsTo_fun in mt; tea. subst. reflexivity.
+          + intros hnin' _. destruct hnin as [hnin _]. specialize (hnin l kl').
+            forward hnin. now left. destruct hnin as [? [hm ?]]. elim hnin'. now exists x. }
+    * destruct H2. eapply H2 in hm as [[kl []]|[hm hkl']] => //.
+      { left. exists kl. split => //. apply H1. now right. intros kl' h. subst k.
+        apply H6. apply H1 in h. destruct h as [[=]|?] => //. subst. congruence. }
+      { right. split => //. intros kl' hin. apply H1 in hin as [[=]|?] => //; subst; try congruence. eauto. }
+Qed.
+
+Lemma min_model_clause_spec l cl a :
+  let map := min_model_clause cl a in
+  is_max_of_clause_map map l cl a.
+Proof.
+  intros m. rewrite /is_max_of_clause_map /is_max_of_clause_model.
+  have h := MapsTo_fold_add_max l (premise cl) (add_max (concl cl) None a).
+  change (LevelExprSet.fold (fun '(l, k0) (acc : model) => add_max l (Some k0) acc) (premise cl)
+      (add_max (concl cl) None a)) with (min_model_clause cl a) in h.
+  cbn in h. destruct h. split.
+  - intros k hm. specialize (H k hm) as [[kl []]|[hm' hle]].
+    * split => //. subst k. red. split. intros kl' hin. constructor. now apply H2.
+      move=> kl' hm''. specialize (H3 kl').
+      rewrite add_max_spec in H3. forward H3.
+      destruct (eq_dec l (concl cl)).
+      { subst l. left. split => //. rewrite max_opt_of_r. apply level_value_MapsTo in hm''. now rewrite hm''. }
+      { right. split => //. }
+      exact H3. left.
+      red. left. red. subst k. eauto.
+    * rewrite add_max_spec in hm'.
+      rewrite max_opt_of_r in hm'. destruct hm' as [[]|[]]; try subst l.
+      { repeat split => //.
+        { intros l hin'. subst k. rewrite (level_value_MapsTo hin'). reflexivity. }
+        { destruct k. right. symmetry in H1. now apply level_value_MapsTo' in H1.
+          left. red. right. split => //. } }
+      { split => //. split => //.
+        { intros l' hin'. eapply LevelMapFact.F.MapsTo_fun in H1; tea. subst. reflexivity. }
+        firstorder. }
+  - intros l' k. destruct H0 as [H0 hext]. specialize (H0 l' k).
+    intros [hm|hinc].
+    { forward H0. left. rewrite add_max_spec.
+      destruct (eq_dec l' (concl cl)); eauto.
+      { left. split => //. rewrite max_opt_of_r.
+        now rewrite (level_value_MapsTo hm). }
+      destruct H0 as [? [hinm hle]].
+      eapply is_higher_mon; tea. exists x. split; eauto. reflexivity. }
+    { red in hinc. destruct hinc. apply H0. now right.
+      destruct H1 as [-> ->].
+      destruct (eq_dec l (concl cl)).
+      red.
+      destruct (LevelMap.find (concl cl) a) eqn:hl.
+      * apply LevelMap.find_2 in hl.
+        specialize (hext (concl cl) o).
+        forward hext. rewrite add_max_spec. left. split => //.
+        rewrite max_opt_of_r. now rewrite (level_value_MapsTo hl).
+        destruct hext as [k' []]. exists k'. split => //. constructor.
+      * specialize (hext (concl cl) None).
+        forward hext. rewrite add_max_spec. left. split => //.
+        now rewrite /level_value hl.
+        destruct cl; unfold clause_conclusion in *. exact hext.
+      * specialize (hext (concl cl) (level_value a (concl cl))).
+        forward hext. rewrite add_max_spec. left. split => //.
+        destruct hext as [l' []]; exists l'; split => //. constructor. }
+Qed.
+
+Lemma min_model_map_acc l cls m :
+  let map := min_model_map m cls in
+  (forall k, LevelMap.MapsTo l k map -> max_of_map l k m) /\
+  m ⩽ map.
+Proof.
+  cbn. rewrite /min_model_map.
+  eapply ClausesProp.fold_rec.
+  2:{ intros. destruct H2 as [hf hin].
+    have [hm hnin] := min_model_clause_spec l x a.
+    split.
+    intros k.
+    move/hm. rewrite /is_max_of_clause_model. intros [[ism' ism] hasm].
+    destruct hasm; eauto. intros kl'. move/hin => [k' [hmk' lek']].
+    red in ism. specialize (ism _ hmk'). now transitivity k'.
+    transitivity a => //.
+    intros l' k ha. specialize (hnin l' k (or_introl ha)).
+    exact hnin. }
+  split; [|reflexivity].
+  intros k hin k' hin'.
+  eapply LevelMapFact.F.MapsTo_fun in hin; tea. subst; reflexivity.
+Qed.
+
+Lemma max_of_map_ext l k m m' : m ⩽ m' -> max_of_map l k m' -> max_of_map l k m.
+Proof.
+  intros hext hm l'; move/hext => [k' [hm' le]].
+  apply hm in hm'. now transitivity k'.
+Qed.
+
+Lemma mapsto_max_of_map l k m : LevelMap.MapsTo l k m -> max_of_map l k m.
+Proof.
+  intros hm l' k'. eapply LevelMapFact.F.MapsTo_fun in hm; tea.
+  subst; reflexivity.
+Qed.
+
+Lemma min_model_map_spec l cls m :
+  let map := min_model_map m cls in
+  (forall k, LevelMap.MapsTo l k map ->
+   [/\ (exists cl, Clauses.In cl cls /\ is_in_clause l k cl) \/ LevelMap.MapsTo l k m,
+    (forall cl, Clauses.In cl cls -> max_of_premises l k (premise cl)) & max_of_map l k m]) /\
+    (forall cl, Clauses.In cl cls -> forall l, LevelSet.In l (clause_levels cl) -> LevelMap.In l map) /\
+    m ⩽ map.
+Proof.
+  cbn.
+  rewrite /min_model_map.
+  have hgen : forall cls m, (forall k, LevelMap.MapsTo l k (Clauses.fold min_model_clause cls m) ->
+    [/\ (exists cl : Clauses.elt, Clauses.In cl cls /\ is_in_clause l k cl) \/
+    LevelMap.MapsTo l k m,
+      forall cl : Clauses.elt, Clauses.In cl cls -> max_of_premises l k (premise cl)
+    & max_of_map l k (Clauses.fold min_model_clause cls m)]) /\
+    (forall cl, Clauses.In cl cls -> forall l, LevelSet.In l (clause_levels cl) -> LevelMap.In l (Clauses.fold min_model_clause cls m)) /\
+    m ⩽ Clauses.fold min_model_clause cls m.
+  2:{ specialize (hgen cls m). destruct hgen as [hgen [hcls H]]; split; eauto.
+      intros k hm. specialize (hgen k hm) as [] => //.
+      split => //. eapply max_of_map_ext; tea. }
+  clear.
+  intros cls m.
+  eapply ClausesProp.fold_rec.
+  - intros s' he. split; [ | split; [|reflexivity]].
+    * intros k hin. split => //. now right.
+      intros cl hin'. clsets. now apply mapsto_max_of_map.
+    * intros cl ins'; clsets.
+  - intros x a s' s'' hin hnin hadd [ih [ihcls hext]]. split; [|split]; revgoals.
+    { transitivity a => //. intros l' hin' hm.
+      have := min_model_clause_spec l' x a. cbn.
+      intros [_ hm']. specialize (hm' l' hin').
+      now forward hm' by eauto. }
+    { intros cl ins'' l' inlev.
+      apply hadd in ins'' as [<-|].
+      * have := min_model_clause_spec l' x a. cbn.
+        intros [_ hm']. eapply clause_levels_spec in inlev as [].
+        + eapply levelexprset_levels_spec in H as [k' incl].
+          specialize (hm' l' (Some k')). forward hm'. right. left. rewrite /is_in_premise. exists k'; eauto.
+          destruct hm' as [? []]; now eexists.
+        + subst l'. specialize (hm' (concl x) None). forward hm'.
+          right. right. split => //.
+          destruct hm' as [? []]; now eexists.
+      * specialize (ihcls _ H _ inlev) as [k' ina].
+        have := min_model_clause_spec l' x a. cbn.
+        move=> [] _ /(_ l' k' (or_introl ina)).
+        clear. firstorder. }
+    intros k.
+    have := min_model_clause_spec l x a. cbn.
+    intros [hm hm'] hmk. destruct (hm _ hmk).
+    split => //.
+    { destruct H0; eauto.
+    { left; exists x. split => //. apply hadd. now left. }
+    { specialize (ih _ H0) as []. destruct H1; eauto. left.
+      move: H1 => [] w []; exists w; split; eauto. apply hadd. now right. } }
+    { move=> cl /hadd => [] [<-|hin'].
+      { now move: H => []. }
+      { specialize (hm' l k). forward hm' by (destruct H0; eauto).
+        intros k' h.
+        specialize (ihcls _ hin' l).
+        forward ihcls.
+        { eapply clause_levels_spec. left. eapply levelexprset_levels_spec. now exists k'. }
+        destruct ihcls as [ka ihcls].
+        specialize (ih _ ihcls) as [ihm ihcls' maxm].
+        specialize (ihcls' _ hin' _ h).
+        transitivity ka => //.
+        destruct H as [mp mmap].
+        now apply mmap. } }
+    { intros kl inma. eapply LevelMapFact.F.MapsTo_fun in hmk; tea. subst. reflexivity. }
+Qed.
+
+Equations? infer_extension {V W init cls} (m : valid_model V W init cls)
+  (hincl : only_model_of V init)
+  (hs : clauses_levels cls ⊂_lset V)
+  (cls' : clauses) :
+  result (LevelSet.union (clauses_levels cls') V) LevelSet.empty (Clauses.union cls cls') (min_model_map m.(model_model) cls') :=
+  infer_extension m hincl hs cls' :=
+    infer_model_extension (LevelSet.union (clauses_levels cls') V) (min_model_map m.(model_model) cls') cls cls' _.
+Proof.
+  repeat split.
+  - lsets.
+  - lsets.
+  - have ms := min_model_map_spec k cls' (model_model m).
+    set (map := min_model_map _ _) in *.
+    destruct ms as [hm [hcls hext]].
+    rewrite LevelSet.union_spec => [] [].
+    * move/clauses_levels_spec.
+      intros [cl [hin ink]].
+      now move: hcls => /(_ _ hin _ ink).
+    * move/(model_of_V m k).
+      move=> [] x /hext. firstorder.
+  - have ms := min_model_map_spec k cls' (model_model m).
+    set (map := min_model_map _ _) in *.
+    destruct ms as [hm [hcls hext]].
+    rewrite LevelSet.union_spec.
+    move=> [] v /hm [] [[cl [incl inclv]]|hm'] ihcls mmap.
+    * left.
+      red in inclv. eapply clauses_levels_spec.
+      exists cl. split => //. eapply clause_levels_spec.
+      destruct inclv as [[? []]|].
+      + left. eapply levelexprset_levels_spec. now eexists.
+      + right. intuition.
+    * have [_ ho] := valid_model_only_model _ _ _ _ m hincl k.
+      forward ho by now exists v. now right.
+Qed.
+
+Lemma only_model_of_min_model_map cls V m :
+  clauses_levels cls ⊂_lset V ->
+  only_model_of V m -> only_model_of V (min_model_map m cls).
+Proof.
+  intros incl om l.
+  split.
+  - move=> /om => [] [k inm].
+    have [hmap [hcls hext]] := min_model_map_spec l cls m.
+    specialize (hext l k inm). firstorder.
+  - have [hmap [hcls hext]] := min_model_map_spec l cls m.
+    move=> [] x /hmap => [] [excl allcl maxm].
+    red in maxm.
+    destruct excl as [[cl [incls incl']]|inm].
+    * apply incl. apply clauses_levels_spec. exists cl. split => //.
+      red in incl'.
+      apply clause_levels_spec.
+      clear -incl'. firstorder. subst. left. apply levelexprset_levels_spec.
+      firstorder.
+    * rewrite (om l). now exists x.
+Qed.
+
+Module CorrectModel.
+  Record t {V cls} :=
+  { the_model : model;
+    only_model_of_V : only_model_of V the_model;
+    model_updates : LevelSet.t;
+    clauses_declared : clauses_levels cls ⊂_lset V;
+    model_valid : valid_model V model_updates the_model cls }.
+  Arguments t : clear implicits.
+
+  #[local] Obligation Tactic := program_simpl.
+  Equations? infer_extension_correct {V W init cls} (m : valid_model V W init cls)
+    (hincl : only_model_of V init)
+    (hs : clauses_levels cls ⊂_lset V)
+    (cls' : clauses)
+    (hs' : clauses_levels cls' ⊂_lset V) : (t V (Clauses.union cls cls')) + premises :=
+  infer_extension_correct m hincl hs cls' hs' with infer_extension m hincl hs cls' :=
+    | Loop u _ => inr u
+    | Model w m' _ =>
+      inl {|
+        the_model := min_model_map m.(model_model) cls';
+        only_model_of_V := _;
+        model_updates := w; clauses_declared := _;
+        model_valid := {| model_model := m'.(model_model) |} |}.
+  Proof.
+    - have := valid_model_only_model _ _ _ _ m hincl.
+      now apply only_model_of_min_model_map.
+    - intros x; rewrite clauses_levels_spec; rw Clauses.union_spec.
+      intros [cl [[hin|hin] incl]]. apply hs. apply clauses_levels_spec. clear -hin incl; firstorder.
+      apply hs'. apply clauses_levels_spec. clear -hin incl; firstorder.
+    - have vm := model_of_V m'. eapply model_of_subset; tea. lsets.
+    - apply m'.
+    - intros ?; rewrite clauses_conclusions_spec.
+      intros [cl [H H']]. apply Clauses.union_spec in H as [H|H];
+        [apply hs|apply hs']; subst a; apply clauses_levels_spec; exists cl; split => //;
+        eapply clause_levels_spec; auto.
+    - apply m'.
+  Qed.
+
+  Equations? infer_extension_valid {V cls} (m : t V cls) cls' : option (t V (Clauses.union cls cls') + premises) :=
+  infer_extension_valid m cls' with inspect (LevelSet.subset (clauses_levels cls') V) :=
+    | exist false heq => None
+    | exist true heq := Some (infer_extension_correct (model_valid m) _ _ cls' _).
+  Proof.
+    - apply only_model_of_V.
+    - now apply m.
+    - now apply LevelSet.subset_spec in heq.
+  Qed.
+End CorrectModel.
+
+Module Abstract.
+  Import CorrectModel.
+  Record t :=
+    { levels : LevelSet.t;
+      clauses : Clauses.t;
+      model : CorrectModel.t levels clauses }.
+
+  Program Definition init_model : t :=
+    {| levels := LevelSet.empty;
+       clauses := Clauses.empty;
+       model := _ |}.
+  Next Obligation.
+    refine {| the_model := LevelMap.empty _;
+      only_model_of_V := _;
+      model_updates := LevelSet.empty; |}.
+    - intros l. split. lsets.
+      intros [x hm]. now eapply LevelMapFact.F.empty_mapsto_iff in hm.
+    - now intros l; rewrite clauses_levels_spec.
+    - refine {| model_model := LevelMap.empty _ |}.
+      * red. lsets.
+      * red. rewrite (proj2 (LevelSet.is_empty_spec _)). lsets.
+        reflexivity.
+      * now intros l; rewrite clauses_conclusions_spec.
+      * rewrite /is_model. eapply Clauses.for_all_spec. tc.
+        intros x hin. now apply Clauses.empty_spec in hin.
+  Qed.
+
+  Equations? declare_level (m : t) (l : Level.t) : option t :=
+  declare_level m l with inspect (LevelSet.mem l m.(levels)) :=
+    | exist true _ => None
+    | exist false hneq => Some {| levels := LevelSet.add l m.(levels); clauses := m.(clauses) |}.
+  Proof.
+    refine {| the_model := LevelMap.add l None m.(model).(the_model);
+      only_model_of_V := _;
+      model_updates := m.(model).(model_updates); |}.
+    - intros k. rewrite LevelSet.add_spec /LevelSet.E.eq.
+      rw LevelMapFact.F.add_mapsto_iff.
+      have hyp := m.(model).(only_model_of_V) k.
+      firstorder; subst. all:rewrite /Level.eq.
+      * now exists None.
+      * exists x. right; split => //. intros ->.
+        apply LevelSetFact.not_mem_iff in hneq. contradiction.
+    - have hyp := m.(model).(clauses_declared). lsets.
+    - destruct m as [levels clauses vm]; cbn in *.
+      destruct vm as [init omofV W incl vm].
+      destruct vm as [M mofV mupd mcls mok]. cbn in *.
+      refine {| model_model := LevelMap.add l None M |}.
+      * intros k. rewrite LevelSet.add_spec LevelMapFact.F.add_in_iff. firstorder. now left.
+      * move: mupd.
+        rewrite /is_update_of.
+        destruct (LevelSet.is_empty) eqn:hw.
+        now intros ->.
+        { apply (todo "strict update weakening"). }
+      * lsets.
+      * apply (todo "cannot activate more clauses").
+  Qed.
+
+  Equations enforce_clauses (m : t) (cls : Clauses.t) : option (t + premises) :=
+  enforce_clauses m cls with infer_extension_valid m.(model) cls :=
+    | None => None
+    | Some (inl m') => Some (inl {| model := m' |})
+    | Some (inr u) => Some (inr u).
+
+End Abstract.
+End Deciders.
+
+Module LoopChecking (LS : LevelSets).
+  Module Impl := Deciders(LS).
+  Import Impl.I.
+
+  Definition model := Impl.Abstract.t.
+
+  Notation univ := LS.LevelExprSet.nonEmptyLevelExprSet.
+
+  Inductive constraint_type := UnivEq | UnivLe.
+  Notation constraint := (univ * constraint_type * univ).
+
+  Definition enforce_constraint (cstr : constraint) (cls : Clauses.t) : Clauses.t :=
+    let '(l, d, r) := cstr in
+    match d with
+    | UnivLe =>
+      LevelExprSet.fold (fun lk acc => Clauses.add (r, lk) acc) (LevelExprSet.t_set l) cls
+    | UnivEq =>
+      let cls :=
+        LevelExprSet.fold (fun lk acc => Clauses.add (r, lk) acc) (LevelExprSet.t_set l) cls
+      in
+      let cls' :=
+        LevelExprSet.fold (fun rk acc => Clauses.add (l, rk) acc) (LevelExprSet.t_set r) cls
+      in cls'
+    end.
+
+  Definition init_model := Impl.Abstract.init_model.
+
+  (* Returns None if already declared *)
+  Definition declare_level l m := Impl.Abstract.declare_level m l.
+
+  (* Returns either a model or a looping universe, i.e. such that u >= u + 1 is implied
+     by the constraint *)
+  Definition enforce c (m : model) : option (model + univ) :=
+    Impl.Abstract.enforce_clauses m (enforce_constraint c Clauses.empty).
+
+  (* Returns true is the clause is valid in the model and all its possible consistent extensions.
+     Returns false if the constraint results in an inconsistent set of constraints or it simply
+     is not valid. *)
+  Definition check m c :=
+    Impl.check_clauses m.(Impl.Abstract.clauses) (enforce_constraint c Clauses.empty).
+
+  (* Returns the valuation of the model: a minimal assignement from levels to constraints
+    that make the enforced clauses valid. *)
+  Definition valuation m := Model.valuation_of_model m.(Impl.Abstract.model).(Impl.CorrectModel.the_model).
+
+End LoopChecking.
